@prefix dc: <http://purl.org/dc/elements/1.1/> .
@prefix dct: <http://purl.org/dc/terms/> .
@prefix dcat: <http://www.w3.org/ns/dcat#> .
@prefix owl: <http://www.w3.org/2002/07/owl#> .
@prefix rdf: <http://www.w3.org/1999/02/22-rdf-syntax-ns#> .
@prefix xsd: <http://www.w3.org/2001/XMLSchema#> .
@prefix prov: <http://www.w3.org/ns/prov#> .
@prefix rdfs: <http://www.w3.org/2000/01/rdf-schema#> .
@prefix skos: <http://www.w3.org/2004/02/skos/core#> .


<http://linked.data.gov.au/def/eudm/agrif>
  rdf:type owl:Ontology ;
  dct:created "2018-06-22"^^xsd:date ;
  dc:creator "Nicholas Car"^^xsd:string ;
  dct:creator <http://orcid.org/0000-0002-8742-7730> ;
  rdfs:comment "This ontology aligns members of the EUDM Profile of the DCAT Ontology with members of the AGRIF Ontology" ;
  rdfs:label "EUDM Profile-AGRIF alignment" ;
  owl:imports <http://linked.data.gov.au/def/agrif> ;
.

#
# Classes
#
dcat:Dataset
  rdfs:subClassOf agrif:Record ;
  dct:description "A Dataset is easily seen as a subclass of Record."@en ;
.

dcat:Distribution
  rdfs:subClassOf agrif:DigitalArtefact ;
  dct:description "Distributions are to Datasets as DigitalArtefacts are to Records, however DigitalArtefacts may not always be associated with a Record thus DigitalArtefact is the superclass."@en ;
.

agrif:Agent
  rdfs:subClassOf foaf:Agent ;
  dct:description "AGRIF implements a stand-alone agrif:Agent class which is \"...responsible for the performance of some Activity or Event, including those on Records\" which means it is clearly a subclass of the generic foaf:Agent class used by DCAT. Note that agrif:Organisation & agrif:Person, subclasses of agrif:Agent have not independent alignment for DCAT given that DCAt only implements foaf:Agent."@en ;
.

dcat:Catalog
  rdfs:subClassOf agrif:InformationSystem ;
  dct:description "AGRIF doesn't specifically mention a Catalog but clearly what DCAT calls a Catalog is a subclass of AGRIF's InformationSystem."@en ;
.

agrif:AGIFTFunction
  rdfs:subClassOf skos:Concept ;
  dct:description "All AGIFT terms are presented as instances of skos:Concepts in the vocabulary https://data.naa.gov.au/def/agift"@en ;
.

agrif:Event
  rdfs:subClassOf prov:InstantaneousEvent ;
  dct:description "AGRIF wording is nearly identical to PROV. This mapping is included (to PROV not DCAT) in order to facilitate inferencing about other events taht might impace DCAT constructs."@en ;
.

# Status is not handled but should be if we use ADMS for lifecycle management

agrif:VersionHistory
  rdfs:subClassOf prov:Bundle ;
    dct:description "A prov:Bundle is a \"a named set of provenance descriptions\"."@en ;

#
# Properties
#
dct:format
  owl:equivalentProperty agrif:format ;
  dct:description "AGRIF's format is defined precicely the same as Dublin Core Terms'."@en ;
.

dcat:byteSize
  rdfs:subPropertyOf agrif:filesize ;
  dct:description "AGRIF's filesize property is clearly similar to dcat:byteSize but the units of measure (bytes v. kiloBytes) are not given."@en ;
.

# agrif:hasClassifier ?

agrif:hasAgent
  skos:narrower prov:agent ;
  dct:description "Since there are no domain or range values for agift:agent, it is unwise to create an inferencing-enabling alignment so SKOS conceptual alignment is used here not RDFS or OWL constructs."@en ;
.

agrif:hasLocation
  rdfs:subPropertyOf prov:atLocation ;
  dct:description "This alignment is to PROV, not DCAT, as DCAT has no property to indicate location (spatial or otherwise) of a resource."@en ;
.

dcat:distribution
  rdfs:subPropertyOf agrif:recordOf ;
  dct:description "This matches the modelling of Record/Dataset and DigitalArtefact/Distribution"@en ;
.

agrif:hasActivity
  rdfs:subPropertyOf prov:used ;
  dct:description "The AGRIF property has no domain or range but usage notes indicate that it is between an Activty and a Record used by it thus, if taken as requirements, domains & range are narrow compared with prov:used."@en ;
.

agrif:hasAgent
  rdfs:subPropertyOf prov:agent ;
  dct:description "The AGRIF property is narrower as it's only to be used through Associations."@en ;
.
