
@prefix rdf: <http://www.w3.org/1999/02/22-rdf-syntax-ns#> .
@prefix rdfs: <http://www.w3.org/2000/01/rdf-schema#> .
@prefix skos: <http://www.w3.org/2004/02/skos/core#> .
@prefix xml: <http://www.w3.org/XML/1998/namespace> .
@prefix xsd: <http://www.w3.org/2001/XMLSchema#> .

<9> a skos:Concept ;
    rdfs:label "National parks, conservation areas, forest reserves and natural water reserves" ;
    skos:topConceptOf <> ;
    skos:narrower <90>,
        <91>,
        <92>,
        <93>,
        <94>,
        <95>,
        <96>,
        <97>,
        <98>,
        <99> ;
    skos:notation "9" ;
    skos:prefLabel "National parks, conservation areas, forest reserves and natural water reserves" .

<Commercial> a skos:Concept ;
    rdfs:label "Commercial" ;
    skos:topConceptOf <> ;
    skos:narrower <20>,
        <21>,
        <22>,
        <23>,
        <24>,
        <25>,
        <26>,
        <27>,
        <28>,
        <29> ;
    skos:notation "2" ;
    skos:prefLabel "Commercial" .

<Community_services> a skos:Concept ;
    rdfs:label "Community services" ;
    skos:topConceptOf <> ;
    skos:narrower <70>,
        <71>,
        <72>,
        <73>,
        <74>,
        <75>,
        <76>,
        <77>,
        <78> ;
    skos:notation "7" ;
    skos:prefLabel "Community services" .

<Extractive_industries> a skos:Concept ;
    rdfs:label "Extractive industries" ;
    skos:topConceptOf <> ;
    skos:narrower <40>,
        <41>,
        <42>,
        <43>,
        <44>,
        <45>,
        <46>,
        <47>,
        <48> ;
    skos:notation "4" ;
    skos:prefLabel "Extractive industries" .

<Industrial> a skos:Concept ;
    rdfs:label "Industrial" ;
    skos:topConceptOf <> ;
    skos:narrower <30>,
        <31>,
        <32>,
        <33> ;
    skos:notation "3" ;
    skos:prefLabel "Industrial" .

<Infrastructure_and_utilities_(industrial)> a skos:Concept ;
    rdfs:label "Infrastructure and utilities (industrial)" ;
    skos:topConceptOf <> ;
    skos:narrower <60>,
        <61>,
        <62>,
        <63>,
        <64>,
        <65>,
        <66>,
        <67>,
        <68>,
        <69> ;
    skos:notation "6" ;
    skos:prefLabel "Infrastructure and utilities (industrial)" .

<Primary_production> a skos:Concept ;
    rdfs:label "Primary production" ;
    skos:topConceptOf <> ;
    skos:narrower <50>,
        <51>,
        <52>,
        <53>,
        <54>,
        <55>,
        <56>,
        <57>,
        <58> ;
    skos:notation "5" ;
    skos:prefLabel "Primary production" .

<Residential> a skos:Concept ;
    rdfs:label "Residential" ;
    skos:topConceptOf <> ;
    skos:narrower <10>,
        <11>,
        <12>,
        <13>,
        <14>,
        <15> ;
    skos:notation "1" ;
    skos:prefLabel "Residential" .

<Sport_Heritage_and_Culture> a skos:Concept ;
    rdfs:label "Sport, Heritage and Culture" ;
    skos:topConceptOf <> ;
    skos:narrower <80>,
        <81>,
        <82>,
        <83>,
        <84>,
        <85> ;
    skos:notation "8" ;
    skos:prefLabel "Sport, Heritage and Culture" .

<10> a skos:Concept ;
    rdfs:label "Residential Use Development Land" ;
    skos:narrower <100>,
        <101>,
        <102>,
        <103>,
        <109> ;
    skos:prefLabel "Residential Use Development Land" .

<100> a skos:Concept ;
    rdfs:label "Vacant Residential Dwelling Site/Surveyed Lot" ;
    skos:definition "Vacant land suitable for the erection of a detached or semi-detached dwelling." ;
    skos:note "Home Changed to Dwelling" ;
    skos:prefLabel "Vacant Residential Dwelling Site/Surveyed Lot" .

<101> a skos:Concept ;
    rdfs:label "Residential Development Site" ;
    skos:definition "Vacant land with a permit approved or capable of being developed for high density residential purposes." ;
    skos:prefLabel "Residential Development Site" .

<102> a skos:Concept ;
    rdfs:label "Vacant In globo Residential Subdivisional Land" ;
    skos:definition "Vacant land zoned for future residential subdivision." ;
    skos:narrower <102.1>,
        <102.2>,
        <102.3> ;
    skos:prefLabel "Vacant In globo Residential Subdivisional Land" .

<102.1> a skos:Concept ;
    rdfs:label "Unspecified" ;
    skos:prefLabel "Unspecified" .

<102.2> a skos:Concept ;
    rdfs:label "Subdivisional Land (Multi Lot)" ;
    skos:prefLabel "Subdivisional Land (Multi Lot)" .

<102.3> a skos:Concept ;
    rdfs:label "Subdivisional Land (In globo/Potential)" ;
    skos:prefLabel "Subdivisional Land (In globo/Potential)" .

<103> a skos:Concept ;
    rdfs:label "Vacant Residential Rural/Rural Lifestyle" ;
    skos:definition "Vacant land in a rural, semi-rural or bushland setting capable of being developed with a single residential dwelling." ;
    skos:prefLabel "Vacant Residential Rural/Rural Lifestyle" .

<109> a skos:Concept ;
    rdfs:label "Residential Airspace" ;
    skos:definition "Airspace capable of being developed for residential purposes, usually above a rooftop, roadway or railway." ;
    skos:prefLabel "Residential Airspace" .

<11> a skos:Concept ;
    rdfs:label "Single Residential Accommodation" ;
    skos:narrower <110>,
        <111>,
        <112>,
        <113>,
        <114>,
        <115>,
        <116>,
        <117>,
        <118> ;
    skos:prefLabel "Single Residential Accommodation" .

<110> a skos:Concept ;
    rdfs:label "Detached Dwelling" ;
    skos:definition "Freestanding dwelling on residential land." ;
    skos:narrower <110.1>,
        <110.2>,
        <110.3>,
        <110.4>,
        <110.5> ;
    skos:note "Home Changed to Dwelling" ;
    skos:prefLabel "Detached Dwelling" .

<110.1> a skos:Concept ;
    rdfs:label "Unspecified" ;
    skos:prefLabel "Unspecified" .

<110.2> a skos:Concept ;
    rdfs:label "Detached Dwelling (new)" ;
    skos:note "Home Changed to Dwelling" ;
    skos:prefLabel "Detached Dwelling (new)" .

<110.3> a skos:Concept ;
    rdfs:label "Detached Dwelling (existing)" ;
    skos:note "Home Changed to Dwelling" ;
    skos:prefLabel "Detached Dwelling (existing)" .

<110.4> a skos:Concept ;
    rdfs:label "Detached Dwelling Non-Conforming Use-Commercial" ;
    skos:definition "Detached dwelling used for residential purposes on commercial land." ;
    skos:note "New AVPCC" ;
    skos:prefLabel "Detached Dwelling Non-Conforming Use-Commercial" .

<110.5> a skos:Concept ;
    rdfs:label "Detached Dwelling Non-Conforming Use-Industrial" ;
    skos:definition "Detached dwelling used for residential purposes on industrial land." ;
    skos:note "New AVPCC" ;
    skos:prefLabel "Detached Dwelling Non-Conforming Use-Industrial" .

<111> a skos:Concept ;
    rdfs:label "Separate Dwelling and Curtilage" ;
    skos:definition "Freestanding dwelling on defined curtilage, being part of a larger holding of varying use, e.g. caretaker’s dwelling on industrial site, second dwelling on farm." ;
    skos:note "Separate House and Curtilage changed to Separate Dwelling and Curtilage" ;
    skos:prefLabel "Separate Dwelling and Curtilage" .

<112> a skos:Concept ;
    rdfs:label "Semi-Detached/Terrace/Row House" ;
    skos:definition "Attached or semi-detached dwelling that does not share common land." ;
    skos:narrower <112.1>,
        <112.2>,
        <112.3>,
        <112.4>,
        <112.5> ;
    skos:note "Semi-Detached/Terrace Home/Row House changed to Semi-Detached/Terrace/Row House" ;
    skos:prefLabel "Semi-Detached/Terrace/Row House" .

<112.1> a skos:Concept ;
    rdfs:label "Unspecified" ;
    skos:prefLabel "Unspecified" .

<112.2> a skos:Concept ;
    rdfs:label "Semi-detached" ;
    skos:prefLabel "Semi-detached" .

<112.3> a skos:Concept ;
    rdfs:label "Terrace" ;
    skos:prefLabel "Terrace" .

<112.4> a skos:Concept ;
    rdfs:label "Row House" ;
    skos:prefLabel "Row House" .

<112.5> a skos:Concept ;
    rdfs:label "Half Pair or Duplex" ;
    skos:prefLabel "Half Pair or Duplex" .

<113> a skos:Concept ;
    rdfs:label "Granny Flat/Studio" ;
    skos:definition "Dwelling either detached or adjoined to a principal dwelling that is self-contained, connected to services but not subdivided in the present form." ;
    skos:prefLabel "Granny Flat/Studio" .

<114> a skos:Concept ;
    rdfs:label "Dwelling and Dependant Unit" ;
    skos:definition "Dwelling and dependant unit not permitted to be separately occupied either detached or adjoined, each self-contained, connected to services but not subdivided in the present form." ;
    skos:note "House and Flat/Studio changed to Dwelling and Dependant Unit" ;
    skos:prefLabel "Dwelling and Dependant Unit" .

<115> a skos:Concept ;
    rdfs:label "Shack/Hut/Donga" ;
    skos:definition "Basic structure with limited services and amenities, providing basic, short-term accommodation." ;
    skos:prefLabel "Shack/Hut/Donga" .

<116> a skos:Concept ;
    rdfs:label "Cabin/Accommodation (rental/leased individual residential site)" ;
    skos:definition "A dwelling subject to a site agreement within a larger complex, e.g. caravan park or lifestyle village. The basis of valuation may vary according to legislation." ;
    skos:prefLabel "Cabin/Accommodation (rental/leased individual residential site)" .

<117> a skos:Concept ;
    rdfs:label "Residential Rural/Rural Lifestyle" ;
    skos:definition "A single residential dwelling on land in a rural, semi-rural or bushland setting.  Primary production uses and associated improvements are secondary to the residential use." ;
    skos:prefLabel "Residential Rural/Rural Lifestyle" .

<118> a skos:Concept ;
    rdfs:label "Residential Land (with buildings that add no value)" ;
    skos:definition "Residential land on which the benefit of works (structures erected) upon the land is exhausted." ;
    skos:prefLabel "Residential Land (with buildings that add no value)" .

<12> a skos:Concept ;
    rdfs:label "Multiple Occupation (within residential development)" ;
    skos:narrower <120>,
        <121>,
        <123>,
        <124>,
        <125>,
        <126>,
        <127>,
        <128>,
        <129> ;
    skos:prefLabel "Multiple Occupation (within residential development)" .

<120> a skos:Concept ;
    rdfs:label "Single Strata Unit/Villa Unit/Townhouse" ;
    skos:definition "Freestanding and unattached unit with ground level footprint." ;
    skos:narrower <120.1>,
        <120.2>,
        <120.3>,
        <120.4>,
        <120.5>,
        <120.6>,
        <120.7> ;
    skos:prefLabel "Single Strata Unit/Villa Unit/Townhouse" .

<120.1> a skos:Concept ;
    rdfs:label "Unspecified" ;
    skos:prefLabel "Unspecified" .

<120.2> a skos:Concept ;
    rdfs:label "Single Strata Unit" ;
    skos:prefLabel "Single Strata Unit" .

<120.3> a skos:Concept ;
    rdfs:label "Villa Unit" ;
    skos:prefLabel "Villa Unit" .

<120.4> a skos:Concept ;
    rdfs:label "Townhouse" ;
    skos:prefLabel "Townhouse" .

<120.5> a skos:Concept ;
    rdfs:label "OYO Subdivided Dwelling" ;
    skos:prefLabel "OYO Subdivided Dwelling" .

<120.6> a skos:Concept ;
    rdfs:label "OYO Subdivided Unit" ;
    skos:prefLabel "OYO Subdivided Unit" .

<120.7> a skos:Concept ;
    rdfs:label "OYO Unit" ;
    skos:prefLabel "OYO Unit" .

<121> a skos:Concept ;
    rdfs:label "Conjoined Strata Unit/Townhouse" ;
    skos:definition "Unit/Townhouse with common walls/party walls with ground level footprint." ;
    skos:narrower <121.1>,
        <121.2>,
        <121.3>,
        <121.4> ;
    skos:prefLabel "Conjoined Strata Unit/Townhouse" .

<121.1> a skos:Concept ;
    rdfs:label "Unspecified" ;
    skos:prefLabel "Unspecified" .

<121.2> a skos:Concept ;
    rdfs:label "Half Pair or Duplex" ;
    skos:prefLabel "Half Pair or Duplex" .

<121.3> a skos:Concept ;
    rdfs:label "Conjoined Strata Unit" ;
    skos:prefLabel "Conjoined Strata Unit" .

<121.4> a skos:Concept ;
    rdfs:label "Townhouse" ;
    skos:prefLabel "Townhouse" .

<123> a skos:Concept ;
    rdfs:label "Residential Company Share Unit (ground level)" ;
    skos:definition "Unit with a ground level footprint where the land is defined by shares in a complex, which gives right to occupy a particular unit. Fully serviced and equipped for long term residential occupation." ;
    skos:narrower <123.1>,
        <123.2>,
        <123.3>,
        <123.4>,
        <123.5>,
        <123.6> ;
    skos:prefLabel "Residential Company Share Unit (ground level)" .

<123.1> a skos:Concept ;
    rdfs:label "Unspecified" ;
    skos:prefLabel "Unspecified" .

<123.2> a skos:Concept ;
    rdfs:label "OYO Company Share Unit" ;
    skos:prefLabel "OYO Company Share Unit" .

<123.3> a skos:Concept ;
    rdfs:label "OYO Stratum Flat" ;
    skos:prefLabel "OYO Stratum Flat" .

<123.4> a skos:Concept ;
    rdfs:label "OYO Stratum Unit" ;
    skos:prefLabel "OYO Stratum Unit" .

<123.5> a skos:Concept ;
    rdfs:label "OYO Company Share Flat" ;
    skos:prefLabel "OYO Company Share Flat" .

<123.6> a skos:Concept ;
    rdfs:label "OYO Cluster Unit" ;
    skos:prefLabel "OYO Cluster Unit" .

<124> a skos:Concept ;
    rdfs:label "Residential Company Share Unit (within multi-storey development)" ;
    skos:definition "Unit which forms part of a multi-storey development where the land is defined by shares in a complex which gives rights to occupy a particular unit. Fully serviced and equipped for long term residential occupation." ;
    skos:prefLabel "Residential Company Share Unit (within multi-storey development)" .

<125> a skos:Concept ;
    rdfs:label "Strata unit or flat" ;
    skos:definition "Unit or flat that forms part of a multi-storey development that has been subdivided." ;
    skos:narrower <125.1>,
        <125.2>,
        <125.3>,
        <125.4> ;
    skos:prefLabel "Strata unit or flat" .

<125.1> a skos:Concept ;
    rdfs:label "Unspecified" ;
    skos:prefLabel "Unspecified" .

<125.2> a skos:Concept ;
    rdfs:label "Strata Dwelling" ;
    skos:prefLabel "Strata Dwelling" .

<125.3> a skos:Concept ;
    rdfs:label "OYO Subdivided Flat" ;
    skos:prefLabel "OYO Subdivided Flat" .

<125.4> a skos:Concept ;
    rdfs:label "OYO Strata Flat" ;
    skos:prefLabel "OYO Strata Flat" .

<126> a skos:Concept ;
    rdfs:label "Individual Car Park" ;
    skos:definition "Individual car park associated with residential use." ;
    skos:prefLabel "Individual Car Park" .

<127> a skos:Concept ;
    rdfs:label "Individual Berth" ;
    skos:definition "Individual berth associated with residential use." ;
    skos:note "New AVPCC" ;
    skos:prefLabel "Individual Berth" .

<128> a skos:Concept ;
    rdfs:label "Individual Flat" ;
    skos:definition "Single flat used for residential purposes within a larger property, e.g. caretakers flat or dwelling above a shop." ;
    skos:note "New AVPCC moved from 132" ;
    skos:prefLabel "Individual Flat" .

<129> a skos:Concept ;
    rdfs:label "Common Land associated with a residential development" ;
    skos:definition "Designated common space, e.g. driveway, gardens or common parking." ;
    skos:prefLabel "Common Land associated with a residential development" .

<13> a skos:Concept ;
    rdfs:label "Investment Residential" ;
    skos:narrower <130>,
        <131>,
        <133>,
        <135> ;
    skos:prefLabel "Investment Residential" .

<130> a skos:Concept ;
    rdfs:label "Boarding House" ;
    skos:definition "Land with a building that is registered to provide long term single room accommodation with shared facilities." ;
    skos:note "Changed from Boarding House/Private Hotel/Dormitory Accommodation/University Residential College to Boarding House" ;
    skos:prefLabel "Boarding House" .

<131> a skos:Concept ;
    rdfs:label "Residential Investment Flats" ;
    skos:definition "A flat that forms part of a complex of two or more flats on land not subdivided." ;
    skos:prefLabel "Residential Investment Flats" .

<133> a skos:Concept ;
    rdfs:label "Short Term Holiday Accommodation" ;
    skos:definition "A residential property used exclusively for short term holiday accommodation for persons away from their normal place of residence." ;
    skos:prefLabel "Short Term Holiday Accommodation" .

<135> a skos:Concept ;
    rdfs:label "Dormitory Accommodation/University Residential College" ;
    skos:definition "Residential accommodation for students usually with shared facilities which is controlled or operated by a registered educational provider." ;
    skos:narrower <135.1>,
        <135.2>,
        <135.3> ;
    skos:note "New AVPCC was previously part of 130" ;
    skos:prefLabel "Dormitory Accommodation/University Residential College" .

<135.1> a skos:Concept ;
    rdfs:label "Unspecified" ;
    skos:prefLabel "Unspecified" .

<135.2> a skos:Concept ;
    rdfs:label "Dormitory Accommodation" ;
    skos:note "New AVPCC" ;
    skos:prefLabel "Dormitory Accommodation" .

<135.3> a skos:Concept ;
    rdfs:label "University Residential College" ;
    skos:note "New AVPCC" ;
    skos:prefLabel "University Residential College" .

<14> a skos:Concept ;
    rdfs:label "Retirement/Aged Care Accommodation/Special Accommodation" ;
    skos:narrower <140>,
        <141>,
        <142>,
        <143>,
        <144> ;
    skos:prefLabel "Retirement/Aged Care Accommodation/Special Accommodation" .

<140> a skos:Concept ;
    rdfs:label "Retirement Village Unit" ;
    skos:definition "Individual unit with self-contained facilities that forms part of retirement village." ;
    skos:prefLabel "Retirement Village Unit" .

<141> a skos:Concept ;
    rdfs:label "Retirement Village Complex" ;
    skos:definition "Land on which a retirement village complex which provides accommodation with shared facilities, amenities and services is erected." ;
    skos:prefLabel "Retirement Village Complex" .

<142> a skos:Concept ;
    rdfs:label "Aged Care Complex" ;
    skos:definition "Land developed with a registered care facility that provides residential accommodation and care services for people, particularly the elderly who can no longer live independently." ;
    skos:narrower <142.1>,
        <142.2>,
        <142.3> ;
    skos:note "Changed from Aged Care Complex/Special Accommodation/Nursing Home to Aged Care Complex" ;
    skos:prefLabel "Aged Care Complex" .

<142.1> a skos:Concept ;
    rdfs:label "Unspecified" ;
    skos:prefLabel "Unspecified" .

<142.2> a skos:Concept ;
    rdfs:label "Aged Care Complex" ;
    skos:prefLabel "Aged Care Complex" .

<142.3> a skos:Concept ;
    rdfs:label "Nursing Home" ;
    skos:prefLabel "Nursing Home" .

<143> a skos:Concept ;
    rdfs:label "Special Accommodation" ;
    skos:definition "Land with residential accommodation provided by registered providers for people with defined medical, social or special support needs." ;
    skos:note "Changed from Aged Care Amenities Buildings to Special Accommodation" ;
    skos:prefLabel "Special Accommodation" .

<144> a skos:Concept ;
    rdfs:label "Disability Housing" ;
    skos:definition "Land on which purpose built housing accommodation for people with disabilities is erected." ;
    skos:prefLabel "Disability Housing" .

<15> a skos:Concept ;
    rdfs:label "Ancillary Buildings" ;
    skos:narrower <150>,
        <151> ;
    skos:prefLabel "Ancillary Buildings" .

<150> a skos:Concept ;
    rdfs:label "Miscellaneous Improvements on Residential Land" ;
    skos:definition "Residential land, on which miscellaneous improvements only are erected, e.g. garages and sheds." ;
    skos:narrower <150.1>,
        <150.2>,
        <150.3> ;
    skos:prefLabel "Miscellaneous Improvements on Residential Land" .

<150.1> a skos:Concept ;
    rdfs:label "Unspecified" ;
    skos:prefLabel "Unspecified" .

<150.2> a skos:Concept ;
    rdfs:label "Storage Area" ;
    skos:prefLabel "Storage Area" .

<150.3> a skos:Concept ;
    rdfs:label "Garage/Outbuilding" ;
    skos:prefLabel "Garage/Outbuilding" .

<151> a skos:Concept ;
    rdfs:label "Miscellaneous Improvements on Residential Rural Land" ;
    skos:definition "Land within a rural, semi-rural or bushland setting and capable of being developed with a single residential dwelling on which miscellaneous improvements only are erected, e.g. garages and sheds." ;
    skos:narrower <151.1>,
        <151.2>,
        <151.3>,
        <151.4> ;
    skos:prefLabel "Miscellaneous Improvements on Residential Rural Land" .

<151.1> a skos:Concept ;
    rdfs:label "Unspecified" ;
    skos:prefLabel "Unspecified" .

<151.2> a skos:Concept ;
    rdfs:label "Storage Area" ;
    skos:prefLabel "Storage Area" .

<151.3> a skos:Concept ;
    rdfs:label "Garage/Outbuilding" ;
    skos:prefLabel "Garage/Outbuilding" .

<151.4> a skos:Concept ;
    rdfs:label "Site Improvements" ;
    skos:prefLabel "Site Improvements" .

<20> a skos:Concept ;
    rdfs:label "Commercial Use Development Land" ;
    skos:narrower <200>,
        <201>,
        <202>,
        <209> ;
    skos:prefLabel "Commercial Use Development Land" .

<200> a skos:Concept ;
    rdfs:label "Commercial Development Site" ;
    skos:definition "Vacant land with a permit approved or capable of being developed for commercial or mixed use purposes." ;
    skos:prefLabel "Commercial Development Site" .

<201> a skos:Concept ;
    rdfs:label "Vacant In globo Commercial Land" ;
    skos:definition "Land which is zoned for future commercial subdivision/development." ;
    skos:prefLabel "Vacant In globo Commercial Land" .

<202> a skos:Concept ;
    rdfs:label "Commercial Land (with buildings that add no value)" ;
    skos:definition "Commercial land on which the benefit of works (structures erected) upon it is exhausted." ;
    skos:prefLabel "Commercial Land (with buildings that add no value)" .

<209> a skos:Concept ;
    rdfs:label "Commercial Airspace" ;
    skos:definition "Airspace capable of being developed for commercial purposes, usually above a rooftop, roadway, railway." ;
    skos:note "Changed from Commercial Development Airspace to Commercial Airspace" ;
    skos:prefLabel "Commercial Airspace" .

<21> a skos:Concept ;
    rdfs:label "Retail" ;
    skos:narrower <210>,
        <211>,
        <212>,
        <213>,
        <214>,
        <215>,
        <216>,
        <217>,
        <218>,
        <219> ;
    skos:prefLabel "Retail" .

<210> a skos:Concept ;
    rdfs:label "Retail Premises (single occupancy)" ;
    skos:definition "Land with retail premises used for the sale of goods or services." ;
    skos:narrower <210.1>,
        <210.2>,
        <210.3>,
        <210.4>,
        <210.5>,
        <210.6>,
        <210.7>,
        <210.8>,
        <210.9> ;
    skos:note "Retail Premises (single occupancy/single title/single stratum) changed to Retail Premises (single occupancy)" ;
    skos:prefLabel "Retail Premises (single occupancy)" .

<210.1> a skos:Concept ;
    rdfs:label "Unspecified" ;
    skos:prefLabel "Unspecified" .

<210.2> a skos:Concept ;
    rdfs:label "Bank" ;
    skos:prefLabel "Bank" .

<210.3> a skos:Concept ;
    rdfs:label "Retail Store/Showroom" ;
    skos:prefLabel "Retail Store/Showroom" .

<210.4> a skos:Concept ;
    rdfs:label "Shop" ;
    skos:prefLabel "Shop" .

<210.5> a skos:Concept ;
    rdfs:label "Café" ;
    skos:prefLabel "Café" .

<210.6> a skos:Concept ;
    rdfs:label "Timber Yard/Trade Supplies" ;
    skos:prefLabel "Timber Yard/Trade Supplies" .

<210.7> a skos:Concept ;
    rdfs:label "Display Yard" ;
    skos:prefLabel "Display Yard" .

<210.8> a skos:Concept ;
    rdfs:label "Convenience Store/Fast Food" ;
    skos:prefLabel "Convenience Store/Fast Food" .

<210.9> a skos:Concept ;
    rdfs:label "Plant/Tree Nursery" ;
    skos:note "New AVPCC" ;
    skos:prefLabel "Plant/Tree Nursery" .

<211> a skos:Concept ;
    rdfs:label "Retail Premises (multiple occupancies)" ;
    skos:definition "Land with more than one retail premises used for the sale of goods or services, regarded as a complex and not subdivided." ;
    skos:narrower <211.1>,
        <211.2>,
        <211.3> ;
    skos:note "Retail Premises (multiple occupancies, usually single title, or the parent title for stratum units) changed to Retail Premises (multiple occupancies)" ;
    skos:prefLabel "Retail Premises (multiple occupancies)" .

<211.1> a skos:Concept ;
    rdfs:label "Unspecified" ;
    skos:prefLabel "Unspecified" .

<211.2> a skos:Concept ;
    rdfs:label "Shop and Dwelling (single occupancy)" ;
    skos:prefLabel "Shop and Dwelling (single occupancy)" .

<211.3> a skos:Concept ;
    rdfs:label "Office and Dwelling (single occupancy)" ;
    skos:prefLabel "Office and Dwelling (single occupancy)" .

<212> a skos:Concept ;
    rdfs:label "Mixed Use Occupation" ;
    skos:definition "Land that includes mixed occupancies, including shops and offices regarded as a complex and not subdivided." ;
    skos:narrower <212.1>,
        <212.3>,
        <212.4>,
        <212.5>,
        <212.6> ;
    skos:prefLabel "Mixed Use Occupation" .

<212.1> a skos:Concept ;
    rdfs:label "Unspecified" ;
    skos:prefLabel "Unspecified" .

<212.3> a skos:Concept ;
    rdfs:label "Office" ;
    skos:note "212.2 Dwelling removed, alternative/s in residential." ;
    skos:prefLabel "Office" .

<212.4> a skos:Concept ;
    rdfs:label "Shop" ;
    skos:prefLabel "Shop" .

<212.5> a skos:Concept ;
    rdfs:label "Studio" ;
    skos:prefLabel "Studio" .

<212.6> a skos:Concept ;
    rdfs:label "Workroom" ;
    skos:prefLabel "Workroom" .

<213> a skos:Concept ;
    rdfs:label "Shopping Centre" ;
    skos:definition "Land developed with a significant retail complex comprising a number of unsubdivided retail premises, parking and associated infrastructure." ;
    skos:narrower <213.1>,
        <213.2>,
        <213.3>,
        <213.4>,
        <213.5>,
        <213.6> ;
    skos:prefLabel "Shopping Centre" .

<213.1> a skos:Concept ;
    rdfs:label "Unspecified" ;
    skos:prefLabel "Unspecified" .

<213.2> a skos:Concept ;
    rdfs:label "Super Regional" ;
    skos:prefLabel "Super Regional" .

<213.3> a skos:Concept ;
    rdfs:label "Major Regional" ;
    skos:prefLabel "Major Regional" .

<213.4> a skos:Concept ;
    rdfs:label "Regional" ;
    skos:prefLabel "Regional" .

<213.5> a skos:Concept ;
    rdfs:label "Sub Regional" ;
    skos:prefLabel "Sub Regional" .

<213.6> a skos:Concept ;
    rdfs:label "Neighbourhood" ;
    skos:prefLabel "Neighbourhood" .

<214> a skos:Concept ;
    rdfs:label "National Company Retail" ;
    skos:definition "Land developed with a purpose built structure and normally occupied by a national company, e.g. supermarket, hardware and home wares." ;
    skos:narrower <214.1>,
        <214.2>,
        <214.3>,
        <214.4> ;
    skos:prefLabel "National Company Retail" .

<214.1> a skos:Concept ;
    rdfs:label "Unspecified" ;
    skos:prefLabel "Unspecified" .

<214.2> a skos:Concept ;
    rdfs:label "Supermarket" ;
    skos:prefLabel "Supermarket" .

<214.3> a skos:Concept ;
    rdfs:label "Department/Discount Department Store" ;
    skos:prefLabel "Department/Discount Department Store" .

<214.4> a skos:Concept ;
    rdfs:label "Bulky Goods" ;
    skos:prefLabel "Bulky Goods" .

<215> a skos:Concept ;
    rdfs:label "Fuel Outlet/Garage/Service Station" ;
    skos:definition "Land used predominantly for fuel sales (multiple pumps) may include car repair and servicing facilities." ;
    skos:prefLabel "Fuel Outlet/Garage/Service Station" .

<216> a skos:Concept ;
    rdfs:label "Multi-Purpose Fuel Outlet (fuel/food/groceries)" ;
    skos:definition "Land used as a service centre usually including fuel sales, retail, restaurant and takeaway food facilities." ;
    skos:prefLabel "Multi-Purpose Fuel Outlet (fuel/food/groceries)" .

<217> a skos:Concept ;
    rdfs:label "Bottle Shop/Licensed Liquor Outlet" ;
    skos:definition "Land developed with a purpose built structure and normally occupied by a national company licensed for the sale of packaged alcohol." ;
    skos:prefLabel "Bottle Shop/Licensed Liquor Outlet" .

<218> a skos:Concept ;
    rdfs:label "Licensed Retail Premises" ;
    skos:definition "Retail premises licensed to sell packaged alcohol." ;
    skos:prefLabel "Licensed Retail Premises" .

<219> a skos:Concept ;
    rdfs:label "Market Stall" ;
    skos:definition "A stall within a market used for the sale of goods and services, e.g. stall at Queen Victoria Market." ;
    skos:prefLabel "Market Stall" .

<22> a skos:Concept ;
    rdfs:label "Office" ;
    skos:narrower <220>,
        <221>,
        <222>,
        <223> ;
    skos:prefLabel "Office" .

<220> a skos:Concept ;
    rdfs:label "Office Premises" ;
    skos:definition "Land used as an office for administration, technical, professional or other like business activity." ;
    skos:narrower <220.1>,
        <220.2>,
        <220.3>,
        <220.4> ;
    skos:note "Changed from Office Premises (single occupancy/single title/single stratum) to Office Premises" ;
    skos:prefLabel "Office Premises" .

<220.1> a skos:Concept ;
    rdfs:label "Unspecified" ;
    skos:prefLabel "Unspecified" .

<220.2> a skos:Concept ;
    rdfs:label "Office (Converted dwelling)" ;
    skos:prefLabel "Office (Converted dwelling)" .

<220.3> a skos:Concept ;
    rdfs:label "Serviced Office" ;
    skos:prefLabel "Serviced Office" .

<220.4> a skos:Concept ;
    rdfs:label "Strata/Subdivided Office" ;
    skos:prefLabel "Strata/Subdivided Office" .

<221> a skos:Concept ;
    rdfs:label "Low Rise Office Building" ;
    skos:definition "Land developed with a 1-3 level office building and used for administration, technical, professional or other like business activity." ;
    skos:prefLabel "Low Rise Office Building" .

<222> a skos:Concept ;
    rdfs:label "Multi-Level Office Building" ;
    skos:definition "Land developed with a 4+ level office building and used for administration, technical, professional or other like business activity." ;
    skos:narrower <222.1>,
        <222.2>,
        <222.3> ;
    skos:prefLabel "Multi-Level Office Building" .

<222.1> a skos:Concept ;
    rdfs:label "Unspecified" ;
    skos:note "New AVPCC - subclassification" ;
    skos:prefLabel "Unspecified" .

<222.2> a skos:Concept ;
    rdfs:label "Medium rise (4 to 50 levels)" ;
    skos:note "New AVPCC - subclassification" ;
    skos:prefLabel "Medium rise (4 to 50 levels)" .

<222.3> a skos:Concept ;
    rdfs:label "High Rise (50+ levels)" ;
    skos:note "New AVPCC - subclassification" ;
    skos:prefLabel "High Rise (50+ levels)" .

<223> a skos:Concept ;
    rdfs:label "Special Purpose (built-in technology)" ;
    skos:definition "Land developed as a purpose-built facility with a high technology component, e.g. call centre." ;
    skos:prefLabel "Special Purpose (built-in technology)" .

<23> a skos:Concept ;
    rdfs:label "Short Term Business and Tourist Accommodation" ;
    skos:narrower <230>,
        <231>,
        <232>,
        <233>,
        <234>,
        <235>,
        <236>,
        <237> ;
    skos:prefLabel "Short Term Business and Tourist Accommodation" .

<230> a skos:Concept ;
    rdfs:label "Residential Hotel/Motel/Apartment Hotel Complex" ;
    skos:definition "Land used to provide accommodation in serviced rooms for persons away from their normal place of residence." ;
    skos:narrower <230.1>,
        <230.2>,
        <230.3>,
        <230.4>,
        <230.5>,
        <230.6>,
        <230.7> ;
    skos:prefLabel "Residential Hotel/Motel/Apartment Hotel Complex" .

<230.1> a skos:Concept ;
    rdfs:label "Unspecified" ;
    skos:prefLabel "Unspecified" .

<230.2> a skos:Concept ;
    rdfs:label "Residential Hotel" ;
    skos:prefLabel "Residential Hotel" .

<230.3> a skos:Concept ;
    rdfs:label "Motel" ;
    skos:prefLabel "Motel" .

<230.4> a skos:Concept ;
    rdfs:label "Apartment Hotel Complex" ;
    skos:prefLabel "Apartment Hotel Complex" .

<230.5> a skos:Concept ;
    rdfs:label "Tourist Resort Complex" ;
    skos:prefLabel "Tourist Resort Complex" .

<230.6> a skos:Concept ;
    rdfs:label "Hotel" ;
    skos:prefLabel "Hotel" .

<230.7> a skos:Concept ;
    rdfs:label "Private Hotel" ;
    skos:note "New AVPCC moved from residential was part of 130" ;
    skos:prefLabel "Private Hotel" .

<231> a skos:Concept ;
    rdfs:label "Residential Hotel/Motel/Apartment Hotel Units" ;
    skos:definition "Subdivided units forming part of a single complex operated as a hotel/motel." ;
    skos:prefLabel "Residential Hotel/Motel/Apartment Hotel Units" .

<232> a skos:Concept ;
    rdfs:label "Serviced Apartments/Holiday Units" ;
    skos:definition "Unit/s within a development used to provide short term accommodation as serviced apartments." ;
    skos:narrower <232.1>,
        <232.2>,
        <232.3> ;
    skos:prefLabel "Serviced Apartments/Holiday Units" .

<232.1> a skos:Concept ;
    rdfs:label "Unspecified" ;
    skos:prefLabel "Unspecified" .

<232.2> a skos:Concept ;
    rdfs:label "Holiday Units" ;
    skos:prefLabel "Holiday Units" .

<232.3> a skos:Concept ;
    rdfs:label "Serviced Apartments" ;
    skos:prefLabel "Serviced Apartments" .

<233> a skos:Concept ;
    rdfs:label "Bed and Breakfast" ;
    skos:definition "Land developed with short-term accommodation, permitted in serviced rooms for persons away from their normal place of residence." ;
    skos:prefLabel "Bed and Breakfast" .

<234> a skos:Concept ;
    rdfs:label "Tourist Park/Caravan Park/Camping Ground" ;
    skos:definition "Land registered as a caravan park and developed with cabins, caravan and camping sites, administration/ablution amenities and recreational facilities." ;
    skos:prefLabel "Tourist Park/Caravan Park/Camping Ground" .

<235> a skos:Concept ;
    rdfs:label "Guest Lodge/Back Packers/Bunkhouse/Hostel" ;
    skos:definition "Land providing basic, short-term residential accommodation usually with shared bathroom and self-service catering facilities." ;
    skos:narrower <235.1>,
        <235.2>,
        <235.3>,
        <235.4> ;
    skos:prefLabel "Guest Lodge/Back Packers/Bunkhouse/Hostel" .

<235.1> a skos:Concept ;
    rdfs:label "Unspecified" ;
    skos:prefLabel "Unspecified" .

<235.2> a skos:Concept ;
    rdfs:label "Guest Lodge" ;
    skos:prefLabel "Guest Lodge" .

<235.3> a skos:Concept ;
    rdfs:label "Back Packers/ Hostel" ;
    skos:prefLabel "Back Packers/ Hostel" .

<235.4> a skos:Concept ;
    rdfs:label "Bunkhouse" ;
    skos:prefLabel "Bunkhouse" .

<236> a skos:Concept ;
    rdfs:label "Ski lodge/ Member facility" ;
    skos:definition "Land developed with short term accommodation for members or guests of a ski lodge/club." ;
    skos:note "New AVPCC" ;
    skos:prefLabel "Ski lodge/ Member facility" .

<237> a skos:Concept ;
    rdfs:label "Recreation Camp" ;
    skos:definition "Land developed with accommodation used by persons or groups for holiday or recreational purposes provided by a commercial operator, e.g. student, youth or family groups." ;
    skos:note "New AVPCC" ;
    skos:prefLabel "Recreation Camp" .

<24> a skos:Concept ;
    rdfs:label "Hospitality" ;
    skos:narrower <240>,
        <241>,
        <242>,
        <243>,
        <244>,
        <245>,
        <246>,
        <247> ;
    skos:prefLabel "Hospitality" .

<240> a skos:Concept ;
    rdfs:label "Pub/Tavern/Hotel/Licensed Club/Restaurant/Licensed Restaurant/Nightclub" ;
    skos:definition "Land licensed to sell liquor but is not permitted to provide gaming facilities. May provide meals, limited accommodation, and/or entertainment." ;
    skos:narrower <240.1>,
        <240.2>,
        <240.3>,
        <240.4>,
        <240.5>,
        <240.6>,
        <240.7>,
        <240.8>,
        <240.9> ;
    skos:prefLabel "Pub/Tavern/Hotel/Licensed Club/Restaurant/Licensed Restaurant/Nightclub" .

<240.1> a skos:Concept ;
    rdfs:label "Unspecified" ;
    skos:prefLabel "Unspecified" .

<240.2> a skos:Concept ;
    rdfs:label "Pub" ;
    skos:prefLabel "Pub" .

<240.3> a skos:Concept ;
    rdfs:label "Tavern" ;
    skos:prefLabel "Tavern" .

<240.4> a skos:Concept ;
    rdfs:label "Hotel" ;
    skos:prefLabel "Hotel" .

<240.5> a skos:Concept ;
    rdfs:label "Licensed Club" ;
    skos:prefLabel "Licensed Club" .

<240.6> a skos:Concept ;
    rdfs:label "Restaurant" ;
    skos:prefLabel "Restaurant" .

<240.7> a skos:Concept ;
    rdfs:label "Licensed Restaurant" ;
    skos:prefLabel "Licensed Restaurant" .

<240.8> a skos:Concept ;
    rdfs:label "Nightclub/Cabaret" ;
    skos:prefLabel "Nightclub/Cabaret" .

<240.9> a skos:Concept ;
    rdfs:label "Reception/Function Centre" ;
    skos:note "Changed from Reception/Function Room to Reception/Function Centre" ;
    skos:prefLabel "Reception/Function Centre" .

<241> a skos:Concept ;
    rdfs:label "Hotel–Gaming" ;
    skos:definition "Land licensed to sell liquor and is permitted to provide gaming facilities. May provide meals, limited accommodation, and/or entertainment." ;
    skos:prefLabel "Hotel–Gaming" .

<242> a skos:Concept ;
    rdfs:label "Club–Gaming – stand alone" ;
    skos:definition "Land permitted to provide gaming facilities associated with a special purpose organisation, e.g. ethnic club, RSL. Access is normally subject to entry conditions." ;
    skos:prefLabel "Club–Gaming – stand alone" .

<243> a skos:Concept ;
    rdfs:label "Member Club Facility" ;
    skos:definition "Land upon which the use of the facilities are restricted by membership requirements. Entry is not available to non-members. May contain any combination of liquor sales, meals and limited accommodation, e.g. RACV member club, The Australian Club." ;
    skos:prefLabel "Member Club Facility" .

<244> a skos:Concept ;
    rdfs:label "Casino" ;
    skos:definition "Land with special operating permit for a large gaming facility." ;
    skos:prefLabel "Casino" .

<245> a skos:Concept ;
    rdfs:label "National Company Restaurant" ;
    skos:definition "Land occupied by a national company and used as a fast food outlet, e.g. KFC, McDonalds." ;
    skos:prefLabel "National Company Restaurant" .

<246> a skos:Concept ;
    rdfs:label "Kiosk" ;
    skos:definition "Land developed with a small retail facility commonly found in public areas, e.g. parks, transport hubs." ;
    skos:prefLabel "Kiosk" .

<247> a skos:Concept ;
    rdfs:label "Conference/Convention centre" ;
    skos:definition "Land developed with purpose built facilities used for conference or convention centre purposes." ;
    skos:note "New AVPCC" ;
    skos:prefLabel "Conference/Convention centre" .

<25> a skos:Concept ;
    rdfs:label "Entertainment – Cinema, Live Theatre and Amusements (non-sporting)" ;
    skos:narrower <250>,
        <251>,
        <252>,
        <253> ;
    skos:prefLabel "Entertainment – Cinema, Live Theatre and Amusements (non-sporting)" .

<250> a skos:Concept ;
    rdfs:label "Live Entertainment – Major Multi-Purpose Complex" ;
    skos:definition "Land developed with a large purpose-built venue used for a wide variety of live entertainment, e.g. Melbourne Arts Centre." ;
    skos:prefLabel "Live Entertainment – Major Multi-Purpose Complex" .

<251> a skos:Concept ;
    rdfs:label "Cinema Complex" ;
    skos:definition "Land developed as a cinema complex incorporating theatres, either stand alone or within a larger complex." ;
    skos:prefLabel "Cinema Complex" .

<252> a skos:Concept ;
    rdfs:label "Playhouse/Traditional Theatre" ;
    skos:definition "Land developed as a theatre, either stand alone or within a larger complex." ;
    skos:prefLabel "Playhouse/Traditional Theatre" .

<253> a skos:Concept ;
    rdfs:label "Drive-In" ;
    skos:definition "Land with an outdoor movie theatre with drive-in parking facilities." ;
    skos:note "Changed from Drive-Ins to Drive-In" ;
    skos:prefLabel "Drive-In" .

<26> a skos:Concept ;
    rdfs:label "Tourism Facilities/Infrastructure" ;
    skos:narrower <260>,
        <261>,
        <262>,
        <263> ;
    skos:prefLabel "Tourism Facilities/Infrastructure" .

<260> a skos:Concept ;
    rdfs:label "Large Theme Attraction/Park" ;
    skos:definition "Land developed as a high profile theme park with attractions, e.g. Sovereign Hill, Ballarat." ;
    skos:note "Changed from Large Theme Attractions/Parks (includes heritage villages etc.) to Large Theme Attraction/Park" ;
    skos:prefLabel "Large Theme Attraction/Park" .

<261> a skos:Concept ;
    rdfs:label "Amusement Park" ;
    skos:definition "Land developed as purpose built amusement park with limited rides and attractions, e.g. Luna Park, Melbourne." ;
    skos:note "Changed from Amusement Parks etc. to Amusement Park" ;
    skos:prefLabel "Amusement Park" .

<262> a skos:Concept ;
    rdfs:label "Major Infrastructure Attractions (often associated with a major historic or feature natural location)." ;
    skos:definition "Land associated with a major tourist attraction destination, e.g. Penguin Parade at Phillip Island, Otway Fly Treetop Walk." ;
    skos:prefLabel "Major Infrastructure Attractions (often associated with a major historic or feature natural location)." .

<263> a skos:Concept ;
    rdfs:label "Tourism Infrastructure – Local Attractions" ;
    skos:definition "Land associated with a local tourist attraction, e.g. cable cars, water slides, chair lifts, tourist railways." ;
    skos:prefLabel "Tourism Infrastructure – Local Attractions" .

<27> a skos:Concept ;
    rdfs:label "Personal Services" ;
    skos:narrower <270>,
        <271>,
        <272>,
        <273>,
        <274>,
        <275> ;
    skos:prefLabel "Personal Services" .

<270> a skos:Concept ;
    rdfs:label "Health Surgery" ;
    skos:definition "Land used by a health practitioner in a stand-alone practice." ;
    skos:prefLabel "Health Surgery" .

<271> a skos:Concept ;
    rdfs:label "Health Clinic" ;
    skos:definition "Land used as consulting suites by health practitioners within an unsubdivided complex, e.g. doctor, chiropractor, dentist, radiologist." ;
    skos:narrower <271.1>,
        <271.2>,
        <271.3>,
        <271.4>,
        <271.5> ;
    skos:prefLabel "Health Clinic" .

<271.1> a skos:Concept ;
    rdfs:label "Unspecified" ;
    skos:prefLabel "Unspecified" .

<271.2> a skos:Concept ;
    rdfs:label "Diagnostic Centre/X-Ray" ;
    skos:prefLabel "Diagnostic Centre/X-Ray" .

<271.3> a skos:Concept ;
    rdfs:label "Medical Centre/Surgery" ;
    skos:prefLabel "Medical Centre/Surgery" .

<271.4> a skos:Concept ;
    rdfs:label "Dental Clinic" ;
    skos:prefLabel "Dental Clinic" .

<271.5> a skos:Concept ;
    rdfs:label "Super Clinic" ;
    skos:prefLabel "Super Clinic" .

<272> a skos:Concept ;
    rdfs:label "Brothel" ;
    skos:definition "Land permitted to be used for the business of providing prostitution services." ;
    skos:prefLabel "Brothel" .

<273> a skos:Concept ;
    rdfs:label "Crematorium/Funeral Services" ;
    skos:definition "Land that is purpose built for undertaking funeral services." ;
    skos:prefLabel "Crematorium/Funeral Services" .

<274> a skos:Concept ;
    rdfs:label "Automatic Teller Machine" ;
    skos:definition "An ATM facility that is not within or attached to banking premises. Can be standalone or separately occupied." ;
    skos:prefLabel "Automatic Teller Machine" .

<275> a skos:Concept ;
    rdfs:label "Veterinary Clinic" ;
    skos:definition "Land used by a veterinary practitioner to treat animals. It may include keeping animals on the premises for treatment or adoption." ;
    skos:prefLabel "Veterinary Clinic" .

<28> a skos:Concept ;
    rdfs:label "Vehicle Car Parking, Washing and Sales" ;
    skos:narrower <280>,
        <281>,
        <282>,
        <283>,
        <284>,
        <285> ;
    skos:prefLabel "Vehicle Car Parking, Washing and Sales" .

<280> a skos:Concept ;
    rdfs:label "Ground Level Parking" ;
    skos:definition "Land used for ground level parking." ;
    skos:prefLabel "Ground Level Parking" .

<281> a skos:Concept ;
    rdfs:label "Multi-Storey Car Park" ;
    skos:definition "Land developed as a multi-storey car parking facility." ;
    skos:prefLabel "Multi-Storey Car Park" .

<282> a skos:Concept ;
    rdfs:label "Individual Car Park Site" ;
    skos:definition "A subdivided car park within a commercial property. Can be leased individually or as part of a single complex by a car park operator." ;
    skos:narrower <282.1>,
        <282.2>,
        <282.3> ;
    skos:prefLabel "Individual Car Park Site" .

<282.1> a skos:Concept ;
    rdfs:label "Unspecified" ;
    skos:prefLabel "Unspecified" .

<282.2> a skos:Concept ;
    rdfs:label "Car park – Under Cover" ;
    skos:prefLabel "Car park – Under Cover" .

<282.3> a skos:Concept ;
    rdfs:label "Car park – Open Air" ;
    skos:prefLabel "Car park – Open Air" .

<283> a skos:Concept ;
    rdfs:label "Car Wash" ;
    skos:definition "Land developed as a purpose built car wash facility. Can be stand alone or part of a larger property." ;
    skos:prefLabel "Car Wash" .

<284> a skos:Concept ;
    rdfs:label "Vehicle Sales Centre" ;
    skos:definition "Land used for the preparation and display of new or second hand vehicles for sale." ;
    skos:prefLabel "Vehicle Sales Centre" .

<285> a skos:Concept ;
    rdfs:label "Vehicle Rental Centre" ;
    skos:definition "Land used for the preparation, storage and display of vehicles available for hire." ;
    skos:note "New AVPCC" ;
    skos:prefLabel "Vehicle Rental Centre" .

<29> a skos:Concept ;
    rdfs:label "Advertising or Public Information Screens" ;
    skos:narrower <290>,
        <293> ;
    skos:prefLabel "Advertising or Public Information Screens" .

<290> a skos:Concept ;
    rdfs:label "Advertising Sign" ;
    skos:definition "Land upon which an advertising sign is erected may be stand alone or form part of a larger property." ;
    skos:narrower <290.1>,
        <290.2>,
        <290.3>,
        <290.4>,
        <290.5> ;
    skos:note "Changed from Static Non Electrical Advertising sign non lighting to Advertising Sign." ;
    skos:prefLabel "Advertising Sign" .

<290.1> a skos:Concept ;
    rdfs:label "Unspecified" ;
    skos:note "New AVPCC - subclassification" ;
    skos:prefLabel "Unspecified" .

<290.2> a skos:Concept ;
    rdfs:label "Self-Standing Pole" ;
    skos:note "New AVPCC - subclassification" ;
    skos:prefLabel "Self-Standing Pole" .

<290.3> a skos:Concept ;
    rdfs:label "Bridge Fixed" ;
    skos:note "New AVPCC - subclassification" ;
    skos:prefLabel "Bridge Fixed" .

<290.4> a skos:Concept ;
    rdfs:label "Roof Mounted" ;
    skos:note "New AVPCC - subclassification" ;
    skos:prefLabel "Roof Mounted" .

<290.5> a skos:Concept ;
    rdfs:label "Wall Fixed" ;
    skos:note "New AVPCC - subclassification" ;
    skos:prefLabel "Wall Fixed" .

<293> a skos:Concept ;
    rdfs:label "Electronic Stadium/Street TV Relay Screen/Scoreboard" ;
    skos:definition "Land upon which electronic screen or scoreboard used for the display of live media and information. May be stand alone or form part of a larger property." ;
    skos:prefLabel "Electronic Stadium/Street TV Relay Screen/Scoreboard" .

<30> a skos:Concept ;
    rdfs:label "Industrial Use Development Land" ;
    skos:narrower <300>,
        <301>,
        <302>,
        <303> ;
    skos:prefLabel "Industrial Use Development Land" .

<300> a skos:Concept ;
    rdfs:label "Industrial Development Site" ;
    skos:definition "Vacant land with a permit approved or capable of being developed for industrial use." ;
    skos:prefLabel "Industrial Development Site" .

<301> a skos:Concept ;
    rdfs:label "Vacant Industrial In globo Land" ;
    skos:definition "Land which is zoned for future industrial subdivision/development." ;
    skos:prefLabel "Vacant Industrial In globo Land" .

<302> a skos:Concept ;
    rdfs:label "Industrial Airspace" ;
    skos:definition "Airspace capable of being developed for industrial purposes, usually above a rooftop, roadway, railway." ;
    skos:prefLabel "Industrial Airspace" .

<303> a skos:Concept ;
    rdfs:label "Industrial Land (with buildings which add no value)" ;
    skos:definition "Industrial land on which the benefit of works (structures erected) upon it is exhausted." ;
    skos:prefLabel "Industrial Land (with buildings which add no value)" .

<31> a skos:Concept ;
    rdfs:label "Manufacturing" ;
    skos:narrower <310>,
        <311>,
        <312> ;
    skos:prefLabel "Manufacturing" .

<310> a skos:Concept ;
    rdfs:label "General Purpose Factory" ;
    skos:definition "Land used for manufacturing, assembly or repairs.  May have specialised/purpose built structures." ;
    skos:narrower <310.1>,
        <310.2>,
        <310.3>,
        <310.4>,
        <310.5>,
        <310.6> ;
    skos:prefLabel "General Purpose Factory" .

<310.1> a skos:Concept ;
    rdfs:label "Unspecified" ;
    skos:prefLabel "Unspecified" .

<310.2> a skos:Concept ;
    rdfs:label "Factory Unit" ;
    skos:prefLabel "Factory Unit" .

<310.3> a skos:Concept ;
    rdfs:label "Factory" ;
    skos:prefLabel "Factory" .

<310.4> a skos:Concept ;
    rdfs:label "Garage/Motor Vehicle Repairs" ;
    skos:prefLabel "Garage/Motor Vehicle Repairs" .

<310.5> a skos:Concept ;
    rdfs:label "Office/Factory" ;
    skos:prefLabel "Office/Factory" .

<310.6> a skos:Concept ;
    rdfs:label "Workshop" ;
    skos:prefLabel "Workshop" .

<311> a skos:Concept ;
    rdfs:label "Food Processing Factory" ;
    skos:definition "Land developed with purpose built food processing facilities, e.g. cannery, milk production plant." ;
    skos:narrower <311.1>,
        <311.2>,
        <311.3> ;
    skos:prefLabel "Food Processing Factory" .

<311.1> a skos:Concept ;
    rdfs:label "Unspecified" ;
    skos:prefLabel "Unspecified" .

<311.2> a skos:Concept ;
    rdfs:label "Processing Plant" ;
    skos:prefLabel "Processing Plant" .

<311.3> a skos:Concept ;
    rdfs:label "Dairy" ;
    skos:prefLabel "Dairy" .

<312> a skos:Concept ;
    rdfs:label "Major Industrial Complex – Special Purpose Improvements" ;
    skos:definition "Land developed with purpose built facilities for large scale industrial use, e.g. car plant, paper mills." ;
    skos:prefLabel "Major Industrial Complex – Special Purpose Improvements" .

<32> a skos:Concept ;
    rdfs:label "Warehouse/Distribution/Storage" ;
    skos:narrower <320>,
        <321>,
        <322>,
        <323>,
        <324>,
        <325>,
        <326> ;
    skos:prefLabel "Warehouse/Distribution/Storage" .

<320> a skos:Concept ;
    rdfs:label "General Purpose Warehouse" ;
    skos:definition "Land used for the storage of goods." ;
    skos:narrower <320.1>,
        <320.2>,
        <320.3>,
        <320.4>,
        <320.5>,
        <320.6>,
        <320.7> ;
    skos:prefLabel "General Purpose Warehouse" .

<320.1> a skos:Concept ;
    rdfs:label "Unspecified" ;
    skos:prefLabel "Unspecified" .

<320.2> a skos:Concept ;
    rdfs:label "Warehouse" ;
    skos:prefLabel "Warehouse" .

<320.3> a skos:Concept ;
    rdfs:label "Warehouse/Office" ;
    skos:prefLabel "Warehouse/Office" .

<320.4> a skos:Concept ;
    rdfs:label "Warehouse/Factory" ;
    skos:prefLabel "Warehouse/Factory" .

<320.5> a skos:Concept ;
    rdfs:label "Warehouse/Showroom" ;
    skos:prefLabel "Warehouse/Showroom" .

<320.6> a skos:Concept ;
    rdfs:label "Depot" ;
    skos:prefLabel "Depot" .

<320.7> a skos:Concept ;
    rdfs:label "Store" ;
    skos:prefLabel "Store" .

<321> a skos:Concept ;
    rdfs:label "Open Area Storage" ;
    skos:definition "Land with extensive hardstand area used for the storage of goods and equipment." ;
    skos:narrower <321.1>,
        <321.2>,
        <321.3>,
        <321.4>,
        <321.5> ;
    skos:prefLabel "Open Area Storage" .

<321.1> a skos:Concept ;
    rdfs:label "Unspecified" ;
    skos:prefLabel "Unspecified" .

<321.2> a skos:Concept ;
    rdfs:label "Hardstand/Storage Yard" ;
    skos:prefLabel "Hardstand/Storage Yard" .

<321.3> a skos:Concept ;
    rdfs:label "Wrecking Yard" ;
    skos:prefLabel "Wrecking Yard" .

<321.4> a skos:Concept ;
    rdfs:label "Concrete Batching Plant" ;
    skos:prefLabel "Concrete Batching Plant" .

<321.5> a skos:Concept ;
    rdfs:label "Container storage" ;
    skos:note "New AVPCC" ;
    skos:prefLabel "Container storage" .

<322> a skos:Concept ;
    rdfs:label "Bulk Grain Storage (structures)" ;
    skos:definition "Land developed with silos used for the storage of grain." ;
    skos:note "Changed from Bulk Grain Storage (structures) to Bulk Grain Storage (structures)" ;
    skos:prefLabel "Bulk Grain Storage (structures)" .

<323> a skos:Concept ;
    rdfs:label "Bulk Grain Storage (earthen walls and flooring - pit bunker)" ;
    skos:definition "Land developed with bunkers used for the storage of grain." ;
    skos:prefLabel "Bulk Grain Storage (earthen walls and flooring - pit bunker)" .

<324> a skos:Concept ;
    rdfs:label "Bulk Liquid Storage Fuel Depot/Tank Farm" ;
    skos:definition "Land developed with tanks for the storage and distribution of bulk liquids, e.g. tank farms, fuel depot." ;
    skos:prefLabel "Bulk Liquid Storage Fuel Depot/Tank Farm" .

<325> a skos:Concept ;
    rdfs:label "Coolstore/Coldstore" ;
    skos:definition "Land with a purpose built structure used for the cold storage of perishable products." ;
    skos:prefLabel "Coolstore/Coldstore" .

<326> a skos:Concept ;
    rdfs:label "Works Depot" ;
    skos:definition "Land developed as a works depot used in conjunction with infrastructure maintenance, e.g. municipal depot." ;
    skos:note "New AVPCC" ;
    skos:prefLabel "Works Depot" .

<33> a skos:Concept ;
    rdfs:label "Noxious/Offensive/Dangerous Industry" ;
    skos:narrower <330>,
        <331>,
        <332>,
        <333>,
        <334>,
        <335>,
        <336> ;
    skos:prefLabel "Noxious/Offensive/Dangerous Industry" .

<330> a skos:Concept ;
    rdfs:label "Tannery/Skins Depot and Drying" ;
    skos:definition "Land developed for the tanning of skins and hides." ;
    skos:prefLabel "Tannery/Skins Depot and Drying" .

<331> a skos:Concept ;
    rdfs:label "Abattoirs" ;
    skos:definition "Land developed with purpose built structures used for the holding and slaughter of stock and the preparation of meat for the wholesale market." ;
    skos:prefLabel "Abattoirs" .

<332> a skos:Concept ;
    rdfs:label "Stock sales yards" ;
    skos:definition "Land developed with purpose built structures used for the yarding and selling of stock." ;
    skos:prefLabel "Stock sales yards" .

<333> a skos:Concept ;
    rdfs:label "Rendering Plant" ;
    skos:definition "Land developed with purpose built structures used for the extraction of lard, tallow, and oil from animal parts." ;
    skos:prefLabel "Rendering Plant" .

<334> a skos:Concept ;
    rdfs:label "Oil Refinery" ;
    skos:definition "Land developed with purpose built structures used in the refinement and storage of petroleum products." ;
    skos:prefLabel "Oil Refinery" .

<335> a skos:Concept ;
    rdfs:label "Petro-chemical Manufacturing" ;
    skos:definition "Land developed with purpose built structures used in the production of chemical based products from petroleum." ;
    skos:prefLabel "Petro-chemical Manufacturing" .

<336> a skos:Concept ;
    rdfs:label "Sawmill" ;
    skos:definition "Land developed with purpose built structures used for the milling and curing of timber." ;
    skos:prefLabel "Sawmill" .

<40> a skos:Concept ;
    rdfs:label "Extractive industry site with permit or reserve not in use" ;
    skos:narrower <400>,
        <401>,
        <402>,
        <403>,
        <404>,
        <405>,
        <406>,
        <407>,
        <408>,
        <409> ;
    skos:prefLabel "Extractive industry site with permit or reserve not in use" .

<400> a skos:Concept ;
    rdfs:label "Sand" ;
    skos:definition "Land permitted to be used, for the extraction of building/manufacture materials (silica)." ;
    skos:prefLabel "Sand" .

<401> a skos:Concept ;
    rdfs:label "Gravel/Stone" ;
    skos:definition "Land permitted to be used, for the extraction of materials used for road works/ construction." ;
    skos:prefLabel "Gravel/Stone" .

<402> a skos:Concept ;
    rdfs:label "Manufacturing Materials" ;
    skos:definition "Land permitted to be used, for the extraction of materials used for manufacturing, such as clay (paper and pottery), Limestone, Dolomite (fertiliser) and Cement/Gypsum (cement)." ;
    skos:prefLabel "Manufacturing Materials" .

<403> a skos:Concept ;
    rdfs:label "Soil" ;
    skos:definition "Land permitted to be used, for the extraction of soil." ;
    skos:prefLabel "Soil" .

<404> a skos:Concept ;
    rdfs:label "Coal" ;
    skos:definition "Land permitted to be used, for the extraction of coal." ;
    skos:prefLabel "Coal" .

<405> a skos:Concept ;
    rdfs:label "Minerals/Ores" ;
    skos:definition "Land permitted to be used, for the extraction of various types of minerals and ore." ;
    skos:prefLabel "Minerals/Ores" .

<406> a skos:Concept ;
    rdfs:label "Precious Metals" ;
    skos:definition "Land permitted to be used, for the extraction of precious metals, e.g. gold, silver." ;
    skos:prefLabel "Precious Metals" .

<407> a skos:Concept ;
    rdfs:label "Uranium" ;
    skos:definition "Land permitted to be used, for the extraction/storage of uranium." ;
    skos:prefLabel "Uranium" .

<408> a skos:Concept ;
    rdfs:label "Quarry/Mine (open cut) – Exhausted (dry)" ;
    skos:definition "Land formerly used for extractive industries whose materials have been exhausted." ;
    skos:prefLabel "Quarry/Mine (open cut) – Exhausted (dry)" .

<409> a skos:Concept ;
    rdfs:label "Quarry/Mine (open cut) – Exhausted (wet)" ;
    skos:definition "Land formerly used for extractive industries whose materials have been exhausted and is now inundated with water." ;
    skos:prefLabel "Quarry/Mine (open cut) – Exhausted (wet)" .

<41> a skos:Concept ;
    rdfs:label "Quarry (in use)" ;
    skos:narrower <410>,
        <411>,
        <412>,
        <413> ;
    skos:prefLabel "Quarry (in use)" .

<410> a skos:Concept ;
    rdfs:label "Sand" ;
    skos:definition "Land from which sand is being extracted by a licensed operator." ;
    skos:prefLabel "Sand" .

<411> a skos:Concept ;
    rdfs:label "Gravel/Stone" ;
    skos:definition "Land from which stone and gravel are being extracted by a licensed operator." ;
    skos:prefLabel "Gravel/Stone" .

<412> a skos:Concept ;
    rdfs:label "Manufacturing Materials" ;
    skos:definition "Land from which manufacturing materials, such as clay (paper and pottery), limestone, dolomite (fertiliser) and cement/gypsum (cement), are being extracted by a licensed operator." ;
    skos:prefLabel "Manufacturing Materials" .

<413> a skos:Concept ;
    rdfs:label "Soil" ;
    skos:definition "Land from which soil is being extracted for by a licensed operator." ;
    skos:prefLabel "Soil" .

<42> a skos:Concept ;
    rdfs:label "Mine (open cut)" ;
    skos:narrower <420>,
        <421>,
        <422>,
        <423>,
        <424>,
        <425>,
        <426>,
        <427> ;
    skos:prefLabel "Mine (open cut)" .

<420> a skos:Concept ;
    rdfs:label "Black or Brown Coal" ;
    skos:definition "Land from which black or brown coal are being extracted by a licensed operator." ;
    skos:prefLabel "Black or Brown Coal" .

<421> a skos:Concept ;
    rdfs:label "Iron Ore" ;
    skos:definition "Land from which iron ore is being extracted by a licensed operator." ;
    skos:prefLabel "Iron Ore" .

<422> a skos:Concept ;
    rdfs:label "Bauxite" ;
    skos:definition "Land from which bauxite is being extracted by a licensed operator." ;
    skos:prefLabel "Bauxite" .

<423> a skos:Concept ;
    rdfs:label "Gold" ;
    skos:definition "Land from which gold is being extracted by a licensed operator." ;
    skos:prefLabel "Gold" .

<424> a skos:Concept ;
    rdfs:label "Metals (other than gold)" ;
    skos:definition "Land from which metals (other than gold) are being extracted by a licensed operator." ;
    skos:prefLabel "Metals (other than gold)" .

<425> a skos:Concept ;
    rdfs:label "Precious Stones" ;
    skos:definition "Land from which precious stones are being extracted for by a licensed operator." ;
    skos:prefLabel "Precious Stones" .

<426> a skos:Concept ;
    rdfs:label "Uranium" ;
    skos:definition "Land from which uranium is being extracted for by a licensed operator." ;
    skos:prefLabel "Uranium" .

<427> a skos:Concept ;
    rdfs:label "Non Metals (other than Uranium)" ;
    skos:definition "Land from which non-metals (other than uranium) being extracted by a licensed operator." ;
    skos:prefLabel "Non Metals (other than Uranium)" .

<43> a skos:Concept ;
    rdfs:label "Mine (deep shaft)" ;
    skos:narrower <430>,
        <431>,
        <432>,
        <433>,
        <434>,
        <439> ;
    skos:prefLabel "Mine (deep shaft)" .

<430> a skos:Concept ;
    rdfs:label "Non-metals" ;
    skos:definition "Land from which non-metals are being extracted by a licensed operator, from deep underground, by way of an inclined or vertical passageway or shaft equipped with lifting machinery." ;
    skos:prefLabel "Non-metals" .

<431> a skos:Concept ;
    rdfs:label "Black Coal" ;
    skos:definition "Land from which black coal is being extracted by a licensed operator from deep underground, by way of an inclined or vertical passageway or shaft equipped with lifting machinery." ;
    skos:prefLabel "Black Coal" .

<432> a skos:Concept ;
    rdfs:label "Precious Stones" ;
    skos:definition "Land from which precious stones are being extracted by a licensed operator from deep underground, by way of an inclined or vertical passageway or shaft equipped with lifting machinery." ;
    skos:prefLabel "Precious Stones" .

<433> a skos:Concept ;
    rdfs:label "Gold" ;
    skos:definition "Land from which gold is being extracted by a licensed operator from deep underground, by way of an inclined or vertical passageway or shaft equipped with lifting machinery." ;
    skos:prefLabel "Gold" .

<434> a skos:Concept ;
    rdfs:label "Metals (other than gold)" ;
    skos:definition "Land from which metals (other than gold) are being extracted by a licensed operator from deep underground, by way of an inclined or vertical passageway or shaft equipped with lifting machinery. Gold may be extracted from ore but it is not the principle mining activity." ;
    skos:prefLabel "Metals (other than gold)" .

<439> a skos:Concept ;
    rdfs:label "Closed Mine Shaft" ;
    skos:definition "Land containing a decommissioned mine shaft, where above ground structures may remain." ;
    skos:prefLabel "Closed Mine Shaft" .

<44> a skos:Concept ;
    rdfs:label "Tailings Dumps" ;
    skos:narrower <440>,
        <441> ;
    skos:prefLabel "Tailings Dumps" .

<440> a skos:Concept ;
    rdfs:label "Tailings Dump (minerals)" ;
    skos:definition "Land permitted to be used for the storage/treatment of minerals in tailing dumps and dams." ;
    skos:prefLabel "Tailings Dump (minerals)" .

<441> a skos:Concept ;
    rdfs:label "Tailings Dump (non-minerals)" ;
    skos:definition "Land permitted to be used for the storage/treatment of non-minerals in tailing dumps and dams." ;
    skos:prefLabel "Tailings Dump (non-minerals)" .

<45> a skos:Concept ;
    rdfs:label "Well/Bore" ;
    skos:narrower <450>,
        <451>,
        <452>,
        <453>,
        <454>,
        <459> ;
    skos:prefLabel "Well/Bore" .

<450> a skos:Concept ;
    rdfs:label "Oil" ;
    skos:definition "Land containing a narrow hole drilled or dug into the earth for the production oil." ;
    skos:prefLabel "Oil" .

<451> a skos:Concept ;
    rdfs:label "Gas" ;
    skos:definition "Land containing a narrow hole drilled or dug into the earth for the production of natural gas." ;
    skos:prefLabel "Gas" .

<452> a skos:Concept ;
    rdfs:label "Water (mineral)" ;
    skos:definition "Land containing a narrow hole drilled or dug into the earth for the production of water (mineral)." ;
    skos:prefLabel "Water (mineral)" .

<453> a skos:Concept ;
    rdfs:label "Water (stock and domestic)" ;
    skos:definition "Land containing a narrow hole drilled or dug into the earth for the production of water, for use for stock and domestic purposes." ;
    skos:prefLabel "Water (stock and domestic)" .

<454> a skos:Concept ;
    rdfs:label "Water (irrigation)" ;
    skos:definition "Land containing a narrow hole drilled or dug into the earth for the production of water, for use in irrigation." ;
    skos:prefLabel "Water (irrigation)" .

<459> a skos:Concept ;
    rdfs:label "Disused Bore/Well" ;
    skos:definition "Land containing a narrow hole drilled into the earth that is decommissioned. Above ground structures may remain." ;
    skos:prefLabel "Disused Bore/Well" .

<46> a skos:Concept ;
    rdfs:label "Salt Pan (evaporative)" ;
    skos:narrower <460>,
        <461> ;
    skos:prefLabel "Salt Pan (evaporative)" .

<460> a skos:Concept ;
    rdfs:label "Lake – Salt Extraction" ;
    skos:definition "Land containing a lake from which salt is extracted." ;
    skos:prefLabel "Lake – Salt Extraction" .

<461> a skos:Concept ;
    rdfs:label "Man-made Evaporative Basin" ;
    skos:definition "Land containing a man-made evaporative basin from which salt is extracted." ;
    skos:prefLabel "Man-made Evaporative Basin" .

<47> a skos:Concept ;
    rdfs:label "Dredging Operations" ;
    skos:narrower <470>,
        <471> ;
    skos:prefLabel "Dredging Operations" .

<470> a skos:Concept ;
    rdfs:label "Dredging (minerals)" ;
    skos:definition "Land on which dredging for the extraction, treatment and restoration of submerged minerals occurs. Usually licensed operations on Crown/State land subject to inundation." ;
    skos:prefLabel "Dredging (minerals)" .

<471> a skos:Concept ;
    rdfs:label "Dredging (non-minerals)" ;
    skos:definition "Land on which dredging for the extraction, treatment and restoration of submerged materials that are not minerals occurs. Usually licensed operations on Crown/State land subject to inundation." ;
    skos:prefLabel "Dredging (non-minerals)" .

<48> a skos:Concept ;
    rdfs:label "Other Unspecified" ;
    skos:narrower <480>,
        <481>,
        <482> ;
    skos:prefLabel "Other Unspecified" .

<480> a skos:Concept ;
    rdfs:label "Extractive less than 2 Metres" ;
    skos:definition "Land from which material is extracted, that do not exceed 2 metres in depth." ;
    skos:prefLabel "Extractive less than 2 Metres" .

<481> a skos:Concept ;
    rdfs:label "Operating mine unspecified" ;
    skos:definition "Land from which material is extracted, but is not otherwise specified." ;
    skos:prefLabel "Operating mine unspecified" .

<482> a skos:Concept ;
    rdfs:label "Vacant Land mining unspecified" ;
    skos:definition "Land from which material has been extracted in the past, that is decommissioned, is vacant land and not otherwise specified." ;
    skos:prefLabel "Vacant Land mining unspecified" .

<50> a skos:Concept ;
    rdfs:label "Native Vegetation" ;
    skos:narrower <500>,
        <501> ;
    skos:prefLabel "Native Vegetation" .

<500> a skos:Concept ;
    rdfs:label "Vacant Land - Native Vegetation/Bushland" ;
    skos:definition "Vacant land that is not cleared with native vegetation coverage typical of the district that is not covered by a covenant or other formal agreement to preserve the vegetation." ;
    skos:note "Changed to Vacant Land - Native Vegetation/Bushland" ;
    skos:prefLabel "Vacant Land - Native Vegetation/Bushland" .

<501> a skos:Concept ;
    rdfs:label "Vacant Land - Native Vegetation/Bushland with Covenant/Agreement" ;
    skos:definition "Vacant land that is not cleared with native vegetation coverage typical of the district, covered by a covenant or other formal agreement to preserve the vegetation." ;
    skos:note "Changed to Vacant Land - Native Vegetation/Bushland with Covenant/Agreement" ;
    skos:prefLabel "Vacant Land - Native Vegetation/Bushland with Covenant/Agreement" .

<51> a skos:Concept ;
    rdfs:label "Agriculture Cropping" ;
    skos:narrower <510>,
        <511> ;
    skos:prefLabel "Agriculture Cropping" .

<510> a skos:Concept ;
    rdfs:label "General Cropping" ;
    skos:definition "Land used for the production of broad-acre crops, e.g. grains, oilseeds and cotton." ;
    skos:narrower <510.1>,
        <510.2>,
        <510.3>,
        <510.4>,
        <510.5> ;
    skos:note "Changed from General Cropping (generally more than 20ha plantings) to General Cropping" ;
    skos:prefLabel "General Cropping" .

<510.1> a skos:Concept ;
    rdfs:label "Unspecified" ;
    skos:prefLabel "Unspecified" .

<510.2> a skos:Concept ;
    rdfs:label "Crop Production – Mixed/Other" ;
    skos:prefLabel "Crop Production – Mixed/Other" .

<510.3> a skos:Concept ;
    rdfs:label "Crop Production – Other Grains/Oil Seeds" ;
    skos:prefLabel "Crop Production – Other Grains/Oil Seeds" .

<510.4> a skos:Concept ;
    rdfs:label "Crop Production – Wheat" ;
    skos:prefLabel "Crop Production – Wheat" .

<510.5> a skos:Concept ;
    rdfs:label "Crop Production – Fodder Crops" ;
    skos:prefLabel "Crop Production – Fodder Crops" .

<511> a skos:Concept ;
    rdfs:label "Specialised Cropping" ;
    skos:definition "Land used in the production of broad-acre crops that require a permit, license or specialist infrastructure, e.g. pyrethrum, poppies." ;
    skos:prefLabel "Specialised Cropping" .

<52> a skos:Concept ;
    rdfs:label "Livestock Grazing" ;
    skos:narrower <520>,
        <521>,
        <522>,
        <523>,
        <524>,
        <525> ;
    skos:prefLabel "Livestock Grazing" .

<520> a skos:Concept ;
    rdfs:label "Domestic Livestock Grazing" ;
    skos:definition "Land used for the grazing of domestic livestock." ;
    skos:prefLabel "Domestic Livestock Grazing" .

<521> a skos:Concept ;
    rdfs:label "Non-Native Animals" ;
    skos:definition "Land used for the grazing of specialist/exotic animals." ;
    skos:prefLabel "Non-Native Animals" .

<522> a skos:Concept ;
    rdfs:label "Native Animals" ;
    skos:definition "Land used for the grazing of native animals." ;
    skos:prefLabel "Native Animals" .

<523> a skos:Concept ;
    rdfs:label "Livestock Production – Sheep" ;
    skos:definition "Land developed with specialist infrastructure and used for the farming of sheep." ;
    skos:prefLabel "Livestock Production – Sheep" .

<524> a skos:Concept ;
    rdfs:label "Livestock Production – Beef Cattle" ;
    skos:definition "Land developed with specialist infrastructure and used for the farming of beef cattle." ;
    skos:prefLabel "Livestock Production – Beef Cattle" .

<525> a skos:Concept ;
    rdfs:label "Livestock Production – Dairy Cattle" ;
    skos:definition "Land developed with specialist infrastructure and used for the farming of dairy cattle." ;
    skos:prefLabel "Livestock Production – Dairy Cattle" .

<53> a skos:Concept ;
    rdfs:label "Mixed Farming and Grazing" ;
    skos:narrower <530> ;
    skos:prefLabel "Mixed Farming and Grazing" .

<530> a skos:Concept ;
    rdfs:label "Mixed farming and grazing" ;
    skos:definition "Land used for mixed use farming purpose, e.g. cropping and grazing/livestock production." ;
    skos:narrower <530.1>,
        <530.2>,
        <530.3> ;
    skos:prefLabel "Mixed farming and grazing" .

<530.1> a skos:Concept ;
    rdfs:label "Unspecified" ;
    skos:prefLabel "Unspecified" .

<530.2> a skos:Concept ;
    rdfs:label "Mixed farming and grazing with infrastructure" ;
    skos:note "Changed from Mixed farming and grazing with structural improvements to farming and grazing with infrastructure" ;
    skos:prefLabel "Mixed farming and grazing with infrastructure" .

<530.3> a skos:Concept ;
    rdfs:label "Mixed farming and grazing without infrastructure" ;
    skos:note "Changed from Mixed farming and grazing without structural improvements to farming and grazing without infrastructure" ;
    skos:prefLabel "Mixed farming and grazing without infrastructure" .

<54> a skos:Concept ;
    rdfs:label "Livestock – special purpose fencing, pens, cages, yards or shedding, stables" ;
    skos:narrower <540>,
        <541>,
        <542>,
        <543>,
        <544>,
        <545>,
        <546> ;
    skos:prefLabel "Livestock – special purpose fencing, pens, cages, yards or shedding, stables" .

<540> a skos:Concept ;
    rdfs:label "Cattle Feed Lot" ;
    skos:definition "Land developed with specialist infrastructure used for intensive feeding of cattle." ;
    skos:prefLabel "Cattle Feed Lot" .

<541> a skos:Concept ;
    rdfs:label "Poultry – Open Range" ;
    skos:definition "Land used for poultry run as free range." ;
    skos:prefLabel "Poultry – Open Range" .

<542> a skos:Concept ;
    rdfs:label "Poultry (egg production)" ;
    skos:definition "Land developed with specialist infrastructure used for egg production." ;
    skos:prefLabel "Poultry (egg production)" .

<543> a skos:Concept ;
    rdfs:label "Poultry (broiler production)" ;
    skos:definition "Land developed with specialist infrastructure used for broiler production." ;
    skos:prefLabel "Poultry (broiler production)" .

<544> a skos:Concept ;
    rdfs:label "Horse Stud/Training Facilities/Stables" ;
    skos:definition "Land developed with specialist infrastructure used as a horse stud farm or horse training facility." ;
    skos:narrower <544.1>,
        <544.2>,
        <544.3>,
        <544.4> ;
    skos:prefLabel "Horse Stud/Training Facilities/Stables" .

<544.1> a skos:Concept ;
    rdfs:label "Unspecified" ;
    skos:prefLabel "Unspecified" .

<544.2> a skos:Concept ;
    rdfs:label "Horse Stud" ;
    skos:prefLabel "Horse Stud" .

<544.3> a skos:Concept ;
    rdfs:label "Training Facilities" ;
    skos:prefLabel "Training Facilities" .

<544.4> a skos:Concept ;
    rdfs:label "Stables" ;
    skos:prefLabel "Stables" .

<545> a skos:Concept ;
    rdfs:label "Piggery" ;
    skos:definition "Land developed with specialist infrastructure for use as a piggery." ;
    skos:prefLabel "Piggery" .

<546> a skos:Concept ;
    rdfs:label "Kennel/Cattery" ;
    skos:definition "Land developed with specialist infrastructure for use as a kennel and/or cattery." ;
    skos:prefLabel "Kennel/Cattery" .

<55> a skos:Concept ;
    rdfs:label "Horticulture Fruit and Vegetable Crops" ;
    skos:narrower <550>,
        <551> ;
    skos:prefLabel "Horticulture Fruit and Vegetable Crops" .

<550> a skos:Concept ;
    rdfs:label "Market Garden – Vegetables" ;
    skos:definition "Land used for the planting of vegetable crops." ;
    skos:note "Changed from Market Garden – Vegetables (generally less than 20ha plantings) to Market Garden – Vegetable" ;
    skos:prefLabel "Market Garden – Vegetables" .

<551> a skos:Concept ;
    rdfs:label "Orchards, Groves and Plantations" ;
    skos:definition "Land used for the planting of trees for the production of fruit and nuts, e.g. olives, stone fruits, tropical fruits, citrus." ;
    skos:prefLabel "Orchards, Groves and Plantations" .

<56> a skos:Concept ;
    rdfs:label "Horticulture – Special Purpose Structural Improvements" ;
    skos:narrower <561>,
        <562>,
        <563>,
        <564> ;
    skos:prefLabel "Horticulture – Special Purpose Structural Improvements" .

<561> a skos:Concept ;
    rdfs:label "Vineyard" ;
    skos:definition "Land developed with specialist infrastructure to facilitate the growing of grapes." ;
    skos:prefLabel "Vineyard" .

<562> a skos:Concept ;
    rdfs:label "Plant/Tree Nursery" ;
    skos:definition "Land used for the propagation, growing and storage of plants." ;
    skos:prefLabel "Plant/Tree Nursery" .

<563> a skos:Concept ;
    rdfs:label "Commercial Flower and Plant Growing – (outdoor)" ;
    skos:definition "Land used for the propagation, growing and storage of flowers and plants." ;
    skos:prefLabel "Commercial Flower and Plant Growing – (outdoor)" .

<564> a skos:Concept ;
    rdfs:label "Glasshouse Plant/Vegetable Production" ;
    skos:definition "Land developed with specialist infrastructure for the indoor propagation and growing of plants and plant crops." ;
    skos:prefLabel "Glasshouse Plant/Vegetable Production" .

<57> a skos:Concept ;
    rdfs:label "Forestry – Commercial Timber Production" ;
    skos:narrower <570>,
        <571>,
        <572> ;
    skos:prefLabel "Forestry – Commercial Timber Production" .

<570> a skos:Concept ;
    rdfs:label "Softwood Plantation" ;
    skos:definition "Land used for the growing and harvesting of softwood trees, e.g. Radiata Pine." ;
    skos:prefLabel "Softwood Plantation" .

<571> a skos:Concept ;
    rdfs:label "Hardwood Plantation" ;
    skos:definition "Land used for the growing and harvesting of hardwood trees, e.g. Blue Gum." ;
    skos:prefLabel "Hardwood Plantation" .

<572> a skos:Concept ;
    rdfs:label "Native Hardwood (standing timber)" ;
    skos:definition "Land used for the growing and harvesting of native trees within a revegetated area." ;
    skos:prefLabel "Native Hardwood (standing timber)" .

<58> a skos:Concept ;
    rdfs:label "Aquaculture" ;
    skos:narrower <580>,
        <581>,
        <582>,
        <583> ;
    skos:prefLabel "Aquaculture" .

<580> a skos:Concept ;
    rdfs:label "Oyster Beds" ;
    skos:definition "Land developed with specialist infrastructure used for the cultivation of oysters." ;
    skos:prefLabel "Oyster Beds" .

<581> a skos:Concept ;
    rdfs:label "Fish Farming – Sea Water Based" ;
    skos:definition "Land developed with specialist infrastructure used for sea-water based fish farming." ;
    skos:prefLabel "Fish Farming – Sea Water Based" .

<582> a skos:Concept ;
    rdfs:label "Yabby Farming" ;
    skos:definition "Land developed with specialist infrastructure used for yabby farming." ;
    skos:prefLabel "Yabby Farming" .

<583> a skos:Concept ;
    rdfs:label "Aquaculture Breeding/Research Facilities/ Fish Hatchery" ;
    skos:definition "Land upon which special purpose aquaculture breeding and/or research facilities are constructed. Includes the breeding and growing of fish for commercial purposes." ;
    skos:prefLabel "Aquaculture Breeding/Research Facilities/ Fish Hatchery" .

<60> a skos:Concept ;
    rdfs:label "Vacant" ;
    skos:narrower <600>,
        <601> ;
    skos:prefLabel "Vacant" .

<600> a skos:Concept ;
    rdfs:label "Vacant Land" ;
    skos:definition "Vacant land reserved or capable of being developed for infrastructure purposes." ;
    skos:prefLabel "Vacant Land" .

<601> a skos:Concept ;
    rdfs:label "Unspecified – Transport, Storage, Utilities and Communication" ;
    skos:definition "Vacant land reserved or capable of being developed for transportation, storage, utilities and communication uses." ;
    skos:prefLabel "Unspecified – Transport, Storage, Utilities and Communication" .

<61> a skos:Concept ;
    rdfs:label "Gas or Fuel" ;
    skos:narrower <610>,
        <611>,
        <612>,
        <613>,
        <614> ;
    skos:note "Changed from Gas to Gas or Fuels" ;
    skos:prefLabel "Gas or Fuel" .

<610> a skos:Concept ;
    rdfs:label "Wells" ;
    skos:definition "Land developed with specialist infrastructure used as a gas or fuel well." ;
    skos:note "Changed from Gas Wells to  Wells" ;
    skos:prefLabel "Wells" .

<611> a skos:Concept ;
    rdfs:label "Production/Refinery" ;
    skos:definition "Land developed with specialist infrastructure used for the production/refinery of gas or fuel." ;
    skos:note "Changed from Gas Production/Refinery to Production/Refinery" ;
    skos:prefLabel "Production/Refinery" .

<612> a skos:Concept ;
    rdfs:label "Storage" ;
    skos:definition "Land developed with specialist infrastructure used for the storage of gas or fuel." ;
    skos:note "Changed from Gas Storage to Storage" ;
    skos:prefLabel "Storage" .

<613> a skos:Concept ;
    rdfs:label "Transmission Pipeline (through easements, freehold and public land)" ;
    skos:definition "Land developed with specialist infrastructure used for the transmission of gas or fuel including pipelines and pressure control facilities." ;
    skos:note "Changed from Gas Transmission Pipeline (through easements, freehold and public land) to Transmission Pipeline (through easements, freehold and public land)" ;
    skos:prefLabel "Transmission Pipeline (through easements, freehold and public land)" .

<614> a skos:Concept ;
    rdfs:label "Distribution/Reticulation Pipelines (through easements, freehold and public land)" ;
    skos:definition "Land developed with specialist infrastructure used for the reticulation of gas or fuel for domestic/commercial purposes." ;
    skos:note "Changed from Gas Distribution/Reticulation Pipelines (through easements, freehold and public land) to Distribution/Reticulation Pipelines (through easements, freehold and public land)" ;
    skos:prefLabel "Distribution/Reticulation Pipelines (through easements, freehold and public land)" .

<62> a skos:Concept ;
    rdfs:label "Electricity" ;
    skos:narrower <620>,
        <621>,
        <622>,
        <623>,
        <624>,
        <625>,
        <626> ;
    skos:prefLabel "Electricity" .

<620> a skos:Concept ;
    rdfs:label "Electricity Power Generators – Fuel Powered (includes brown coal, black coal, natural steam, gas, oil and nuclear)" ;
    skos:definition "Land developed with specialist infrastructure used in the generation of fossil fuelled electricity." ;
    skos:prefLabel "Electricity Power Generators – Fuel Powered (includes brown coal, black coal, natural steam, gas, oil and nuclear)" .

<621> a skos:Concept ;
    rdfs:label "Hydroelectricity Generation" ;
    skos:definition "Land developed with specialist infrastructure used in the generation of hydroelectricity." ;
    skos:prefLabel "Hydroelectricity Generation" .

<622> a skos:Concept ;
    rdfs:label "Wind Farm Electricity Generation" ;
    skos:definition "Land developed with specialist infrastructure used in the generation of wind powered electricity." ;
    skos:prefLabel "Wind Farm Electricity Generation" .

<623> a skos:Concept ;
    rdfs:label "Electricity Substation/Terminal" ;
    skos:definition "Land developed with specialist infrastructure associated with the reticulation of electricity." ;
    skos:prefLabel "Electricity Substation/Terminal" .

<624> a skos:Concept ;
    rdfs:label "Electricity Transmission Lines (through easements, freehold and public land)" ;
    skos:definition "Land developed with transmission lines used for electricity transmission." ;
    skos:prefLabel "Electricity Transmission Lines (through easements, freehold and public land)" .

<625> a skos:Concept ;
    rdfs:label "Electricity Distribution/Reticulation Lines (through easements, freehold and public land)" ;
    skos:definition "Land developed with specialist infrastructure with a transmission line used for domestic/commercial reticulation." ;
    skos:prefLabel "Electricity Distribution/Reticulation Lines (through easements, freehold and public land)" .

<626> a skos:Concept ;
    rdfs:label "Solar Electricity Generation" ;
    skos:definition "Land developed with specialist infrastructure used in the generation of solar electricity." ;
    skos:note "New AVPCC" ;
    skos:prefLabel "Solar Electricity Generation" .

<63> a skos:Concept ;
    rdfs:label "Waste Disposal, Treatment and Recycling" ;
    skos:narrower <630>,
        <631>,
        <632>,
        <633>,
        <634>,
        <635>,
        <636>,
        <637>,
        <638> ;
    skos:prefLabel "Waste Disposal, Treatment and Recycling" .

<630> a skos:Concept ;
    rdfs:label "Refuse Incinerator" ;
    skos:definition "Land developed with specialist infrastructure used for the incineration of refuse." ;
    skos:prefLabel "Refuse Incinerator" .

<631> a skos:Concept ;
    rdfs:label "Refuse Transfer Station" ;
    skos:definition "Land developed with specialist infrastructure used in the storage and transfer of refuse." ;
    skos:prefLabel "Refuse Transfer Station" .

<632> a skos:Concept ;
    rdfs:label "Sanitary Land Fill" ;
    skos:definition "Land permitted to be used for the disposal of household, commercial, industrial and public waste." ;
    skos:prefLabel "Sanitary Land Fill" .

<633> a skos:Concept ;
    rdfs:label "Refuse Recycling" ;
    skos:definition "Land developed with specialist infrastructure used in the recycling of refuse." ;
    skos:prefLabel "Refuse Recycling" .

<634> a skos:Concept ;
    rdfs:label "Hazardous Materials/Toxic Storage Centre" ;
    skos:definition "Land permitted to be used for the storage of hazardous materials and toxic waste." ;
    skos:prefLabel "Hazardous Materials/Toxic Storage Centre" .

<635> a skos:Concept ;
    rdfs:label "Toxic By-product Storage and Decontamination Site" ;
    skos:definition "Land permitted to be used for the storage of mining waste." ;
    skos:prefLabel "Toxic By-product Storage and Decontamination Site" .

<636> a skos:Concept ;
    rdfs:label "Sewerage/Stormwater Treatment Plant Site" ;
    skos:definition "Land developed with specialist infrastructure used in the treatment of sewerage and stormwater." ;
    skos:prefLabel "Sewerage/Stormwater Treatment Plant Site" .

<637> a skos:Concept ;
    rdfs:label "Sewerage/Stormwater Pump Stations" ;
    skos:definition "Land developed with specialist infrastructure used in the pumping of sewerage and stormwater." ;
    skos:prefLabel "Sewerage/Stormwater Pump Stations" .

<638> a skos:Concept ;
    rdfs:label "Sewerage/Stormwater Pipelines (through easements, freehold and public land)" ;
    skos:definition "Land developed with pipelines or channels used for domestic sewerage or stormwater reticulation." ;
    skos:narrower <638.1>,
        <638.2>,
        <638.3>,
        <638.4>,
        <638.5> ;
    skos:prefLabel "Sewerage/Stormwater Pipelines (through easements, freehold and public land)" .

<638.1> a skos:Concept ;
    rdfs:label "Unspecified" ;
    skos:prefLabel "Unspecified" .

<638.2> a skos:Concept ;
    rdfs:label "Public Utility – Drainage" ;
    skos:prefLabel "Public Utility – Drainage" .

<638.3> a skos:Concept ;
    rdfs:label "Public Utility – Sewerage" ;
    skos:prefLabel "Public Utility – Sewerage" .

<638.4> a skos:Concept ;
    rdfs:label "Reserve for Drainage or Sewerage Purposes" ;
    skos:note "Changed from Reserve for Drainage Purposes to Reserve for Drainage or sewerage Purposes" ;
    skos:prefLabel "Reserve for Drainage or Sewerage Purposes" .

<638.5> a skos:Concept ;
    rdfs:label "Retarding Basin" ;
    skos:note "New AVPCC" ;
    skos:prefLabel "Retarding Basin" .

<64> a skos:Concept ;
    rdfs:label "Water Supply" ;
    skos:narrower <640>,
        <641>,
        <642>,
        <643>,
        <644>,
        <645>,
        <646> ;
    skos:prefLabel "Water Supply" .

<640> a skos:Concept ;
    rdfs:label "Water Catchment Area" ;
    skos:definition "Land used for the purpose of water catchment within a designated water catchment area." ;
    skos:prefLabel "Water Catchment Area" .

<641> a skos:Concept ;
    rdfs:label "Water Catchment Dam/Reservoir" ;
    skos:definition "Land developed with specialist infrastructure and used as a dam, weir, storage basin or reservoir for water catchment." ;
    skos:prefLabel "Water Catchment Dam/Reservoir" .

<642> a skos:Concept ;
    rdfs:label "Water Storage Dam/Reservoir (Non-Catchment)" ;
    skos:definition "Land developed with specialist infrastructure and used as a dam, weir, storage basin or reservoir for water storage." ;
    skos:prefLabel "Water Storage Dam/Reservoir (Non-Catchment)" .

<643> a skos:Concept ;
    rdfs:label "Water Treatment Plant" ;
    skos:definition "Land developed with specialist infrastructure used for the treatment of water, e.g. desalination plant." ;
    skos:prefLabel "Water Treatment Plant" .

<644> a skos:Concept ;
    rdfs:label "Water Storage Tanks, Pressure Control Towers and Pumping Stations." ;
    skos:definition "Land developed with water storage tanks, pressure control towers and pumping stations used for water supply." ;
    skos:prefLabel "Water Storage Tanks, Pressure Control Towers and Pumping Stations." .

<645> a skos:Concept ;
    rdfs:label "Major Water Conduits" ;
    skos:definition "Land developed with canals, flumes, pipes to carry water to power stations, treatment plants and irrigation supply channels used for the supply of water." ;
    skos:prefLabel "Major Water Conduits" .

<646> a skos:Concept ;
    rdfs:label "Water – Urban Distribution Network (through easements, freehold and public land)" ;
    skos:definition "Land developed with infrastructure for the domestic reticulation of water." ;
    skos:prefLabel "Water – Urban Distribution Network (through easements, freehold and public land)" .

<65> a skos:Concept ;
    rdfs:label "Transport – Road Systems" ;
    skos:narrower <650>,
        <651>,
        <652>,
        <653>,
        <654>,
        <655>,
        <656>,
        <657>,
        <658>,
        <659> ;
    skos:prefLabel "Transport – Road Systems" .

<650> a skos:Concept ;
    rdfs:label "Freeways" ;
    skos:definition "Land that forms part of a freeway." ;
    skos:prefLabel "Freeways" .

<651> a skos:Concept ;
    rdfs:label "Main Highways (including national routes)" ;
    skos:definition "Land that forms part of a main highway." ;
    skos:prefLabel "Main Highways (including national routes)" .

<652> a skos:Concept ;
    rdfs:label "Secondary Roads" ;
    skos:definition "Land that forms part of a secondary road." ;
    skos:prefLabel "Secondary Roads" .

<653> a skos:Concept ;
    rdfs:label "Suburban and Rural Roads" ;
    skos:definition "Land that forms part of a suburban or rural road." ;
    skos:prefLabel "Suburban and Rural Roads" .

<654> a skos:Concept ;
    rdfs:label "Closed Roads" ;
    skos:definition "Land that forms part of a road that is now closed." ;
    skos:prefLabel "Closed Roads" .

<655> a skos:Concept ;
    rdfs:label "Reserved Roads" ;
    skos:definition "Land reserved for future roads." ;
    skos:note "Changed from Reserved Roads/Unused Roads to Reserved Roads" ;
    skos:prefLabel "Reserved Roads" .

<656> a skos:Concept ;
    rdfs:label "Bus Maintenance Depot" ;
    skos:definition "Land developed for the parking and maintenance of passenger buses." ;
    skos:prefLabel "Bus Maintenance Depot" .

<657> a skos:Concept ;
    rdfs:label "Bus Interchange Centre/Bus Terminal" ;
    skos:definition "Land developed as a bus interchange centre/bus terminal." ;
    skos:prefLabel "Bus Interchange Centre/Bus Terminal" .

<658> a skos:Concept ;
    rdfs:label "Designated Bus/Taxi Stops/Stands/Shelters" ;
    skos:definition "Land developed as a bus/taxi stop. Includes designated areas, stands and shelters." ;
    skos:prefLabel "Designated Bus/Taxi Stops/Stands/Shelters" .

<659> a skos:Concept ;
    rdfs:label "Weighbridge" ;
    skos:definition "Land developed with a weighbridge." ;
    skos:prefLabel "Weighbridge" .

<66> a skos:Concept ;
    rdfs:label "Transport – Rail and Tramway Systems" ;
    skos:narrower <660>,
        <661>,
        <662>,
        <663>,
        <664>,
        <665>,
        <666>,
        <667>,
        <668> ;
    skos:prefLabel "Transport – Rail and Tramway Systems" .

<660> a skos:Concept ;
    rdfs:label "Railway Line in use" ;
    skos:definition "Land developed and used as an operating railway line and associated infrastructure." ;
    skos:note "Changed from Railway Line Land and Improvements in use to Railway Line in use" ;
    skos:prefLabel "Railway Line in use" .

<661> a skos:Concept ;
    rdfs:label "Railway Switching and Marshalling Yards" ;
    skos:definition "Land developed and used as a railway switching and marshalling yard." ;
    skos:prefLabel "Railway Switching and Marshalling Yards" .

<662> a skos:Concept ;
    rdfs:label "Railway Maintenance Facility" ;
    skos:definition "Land developed and used for railway maintenance." ;
    skos:prefLabel "Railway Maintenance Facility" .

<663> a skos:Concept ;
    rdfs:label "Railway Passenger Terminal Facilities (including stations)" ;
    skos:definition "Land developed and used as a railway passenger terminal." ;
    skos:note "Changed from Railway Passenger Terminal Facilities (including stations etc.) to Railway Passenger Terminal Facilities (including stations)" ;
    skos:prefLabel "Railway Passenger Terminal Facilities (including stations)" .

<664> a skos:Concept ;
    rdfs:label "Railway Freight Terminal Facilities" ;
    skos:definition "Land developed and used as a railway freight terminal." ;
    skos:prefLabel "Railway Freight Terminal Facilities" .

<665> a skos:Concept ;
    rdfs:label "Tramway/Light Rail Right of Way and Associated Track Infrastructure" ;
    skos:definition "Land developed and used as an operating tram or light rail service and associated infrastructure." ;
    skos:note "Changed from Tramway/Light Rail Right of Way and Associated Track Improvements to Tramway/Light Rail Right of Way and Associated Track Infrastructure" ;
    skos:prefLabel "Tramway/Light Rail Right of Way and Associated Track Infrastructure" .

<666> a skos:Concept ;
    rdfs:label "Tramway Maintenance /Terminal Storage" ;
    skos:definition "Land developed and used for tramway maintenance and terminal facilities." ;
    skos:prefLabel "Tramway Maintenance /Terminal Storage" .

<667> a skos:Concept ;
    rdfs:label "Tram Stopping Facilities" ;
    skos:definition "Land developed and used for a tram stop. Includes shelters and platforms." ;
    skos:prefLabel "Tram Stopping Facilities" .

<668> a skos:Concept ;
    rdfs:label "Railway/Tramway Line Closed/Unused" ;
    skos:definition "Land developed and no longer used for tramways or other related facilities." ;
    skos:prefLabel "Railway/Tramway Line Closed/Unused" .

<67> a skos:Concept ;
    rdfs:label "Transport – Air" ;
    skos:narrower <670>,
        <671>,
        <672>,
        <673>,
        <674>,
        <675>,
        <676> ;
    skos:prefLabel "Transport – Air" .

<670> a skos:Concept ;
    rdfs:label "Airfield (includes associated open space)" ;
    skos:definition "Land developed with specialist infrastructure used as an airport capable of handling domestic and/or international services." ;
    skos:prefLabel "Airfield (includes associated open space)" .

<671> a skos:Concept ;
    rdfs:label "Airstrip" ;
    skos:definition "Land developed with limited infrastructure and used as a local/regional airstrip." ;
    skos:prefLabel "Airstrip" .

<672> a skos:Concept ;
    rdfs:label "Airport Traffic Control Centre" ;
    skos:definition "Land developed with specialist infrastructure used and operated as an air traffic control centre." ;
    skos:prefLabel "Airport Traffic Control Centre" .

<673> a skos:Concept ;
    rdfs:label "Airport Hangar Building" ;
    skos:definition "Land developed with specialist infrastructure used for aircraft maintenance and storage." ;
    skos:prefLabel "Airport Hangar Building" .

<674> a skos:Concept ;
    rdfs:label "Airport Terminal Building – Passengers" ;
    skos:definition "Land developed with specialist infrastructure used in conjunction with airline operations to manage passenger services." ;
    skos:prefLabel "Airport Terminal Building – Passengers" .

<675> a skos:Concept ;
    rdfs:label "Airport Terminal Building – Freight" ;
    skos:definition "Land developed with specialist infrastructure used for freight handling services within an airport." ;
    skos:prefLabel "Airport Terminal Building – Freight" .

<676> a skos:Concept ;
    rdfs:label "Heliport" ;
    skos:definition "Land developed and used for helicopter landing and parking." ;
    skos:prefLabel "Heliport" .

<68> a skos:Concept ;
    rdfs:label "Transport – Marine" ;
    skos:narrower <680>,
        <681>,
        <682>,
        <683>,
        <684>,
        <685>,
        <686>,
        <687>,
        <688>,
        <689> ;
    skos:prefLabel "Transport – Marine" .

<680> a skos:Concept ;
    rdfs:label "Port Channel" ;
    skos:definition "Designated channel used as a shipping waterway." ;
    skos:prefLabel "Port Channel" .

<681> a skos:Concept ;
    rdfs:label "Port Dock/Berth" ;
    skos:definition "Seabed adjoining a wharf and developed with infrastructure used for the berthing of ships." ;
    skos:prefLabel "Port Dock/Berth" .

<682> a skos:Concept ;
    rdfs:label "Port Wharf/Pier and Apron – Cargo" ;
    skos:definition "Land developed with specialist infrastructure to facilitate the movement of containers and cargo to and from ships." ;
    skos:prefLabel "Port Wharf/Pier and Apron – Cargo" .

<683> a skos:Concept ;
    rdfs:label "Wharf – Storage Sheds" ;
    skos:definition "Land developed with enclosed storage facilities within a wharf." ;
    skos:prefLabel "Wharf – Storage Sheds" .

<684> a skos:Concept ;
    rdfs:label "Wharf – Passenger Terminal and Ferry Pier Facilities" ;
    skos:definition "Land developed with passenger terminals and other facilities within a wharf or pier." ;
    skos:prefLabel "Wharf – Passenger Terminal and Ferry Pier Facilities" .

<685> a skos:Concept ;
    rdfs:label "Piers, Storages and Slipways" ;
    skos:definition "Land developed and used for the maintenance and launching of boats." ;
    skos:prefLabel "Piers, Storages and Slipways" .

<686> a skos:Concept ;
    rdfs:label "Ramps and Jetties" ;
    skos:definition "Land developed with limited infrastructure used for recreational boating purposes." ;
    skos:note "Changed from Boat Sheds, Bathing Boxes, Ramps and Jetties to  Ramps and Jetties" ;
    skos:prefLabel "Ramps and Jetties" .

<687> a skos:Concept ;
    rdfs:label "Marinas and Yacht Clubs" ;
    skos:definition "Land developed with specialist infrastructure used for the wet and dry storage of leisure boats." ;
    skos:prefLabel "Marinas and Yacht Clubs" .

<688> a skos:Concept ;
    rdfs:label "Dockyard, Dry Dock and/or Ship Building Facility" ;
    skos:definition "Land developed with specialist infrastructure used for the repair, maintenance, and construction of ships." ;
    skos:prefLabel "Dockyard, Dry Dock and/or Ship Building Facility" .

<689> a skos:Concept ;
    rdfs:label "Lighthouse and Navigation Aids" ;
    skos:definition "Land developed with specialist infrastructure used to assist in sea navigation." ;
    skos:prefLabel "Lighthouse and Navigation Aids" .

<69> a skos:Concept ;
    rdfs:label "Communications, including Print, Post, Telecommunications and Airwave Facilities" ;
    skos:narrower <690>,
        <691>,
        <692>,
        <693>,
        <694>,
        <695>,
        <696>,
        <697>,
        <698> ;
    skos:prefLabel "Communications, including Print, Post, Telecommunications and Airwave Facilities" .

<690> a skos:Concept ;
    rdfs:label "Post Offices" ;
    skos:definition "Land used for the collection/ distribution of mail and the sale of products associated with that use." ;
    skos:prefLabel "Post Offices" .

<691> a skos:Concept ;
    rdfs:label "Postal Exchange/Mail Sorting Centres" ;
    skos:definition "Land developed and used for the sorting of mail." ;
    skos:prefLabel "Postal Exchange/Mail Sorting Centres" .

<692> a skos:Concept ;
    rdfs:label "Post Boxes" ;
    skos:definition "Land developed with a single receptacle for the posting of mail." ;
    skos:prefLabel "Post Boxes" .

<693> a skos:Concept ;
    rdfs:label "Telecommunication Buildings/Maintenance Depots" ;
    skos:definition "Land developed and used for the maintenance of telecommunication installations." ;
    skos:prefLabel "Telecommunication Buildings/Maintenance Depots" .

<694> a skos:Concept ;
    rdfs:label "Telecommunication Towers and Aerials" ;
    skos:definition "Land developed with specialist infrastructure used for the transmission of telecommunication signals. Maybe be stand alone or affixed to buildings." ;
    skos:narrower <694.1>,
        <694.2>,
        <694.3> ;
    skos:prefLabel "Telecommunication Towers and Aerials" .

<694.1> a skos:Concept ;
    rdfs:label "Unspecified" ;
    skos:prefLabel "Unspecified" .

<694.2> a skos:Concept ;
    rdfs:label "Telecommunication Tower" ;
    skos:prefLabel "Telecommunication Tower" .

<694.3> a skos:Concept ;
    rdfs:label "Telecommunication Aerial" ;
    skos:prefLabel "Telecommunication Aerial" .

<695> a skos:Concept ;
    rdfs:label "Cable Lines, Conduits and Special Purpose Below Street Level Communication Line Tunnels – not being sewers (through easements, freehold and public land)" ;
    skos:definition "Land developed with cable lines, conduits and special purpose, below street level and communication line tunnels used for telecommunication purposes." ;
    skos:prefLabel "Cable Lines, Conduits and Special Purpose Below Street Level Communication Line Tunnels – not being sewers (through easements, freehold and public land)" .

<696> a skos:Concept ;
    rdfs:label "Television/Radio Station – Purpose Built" ;
    skos:definition "Land developed with specialist infrastructure used for the production/ recording of television and radio programs." ;
    skos:prefLabel "Television/Radio Station – Purpose Built" .

<697> a skos:Concept ;
    rdfs:label "Printing Works/Press" ;
    skos:definition "Land developed with specialist infrastructure and used for printing works, e.g. newspaper print, magazines." ;
    skos:prefLabel "Printing Works/Press" .

<698> a skos:Concept ;
    rdfs:label "Telephone Exchange – Purpose Built" ;
    skos:definition "Land developed with specialist infrastructure used to facilitate the transmission of telephonics." ;
    skos:prefLabel "Telephone Exchange – Purpose Built" .

<70> a skos:Concept ;
    rdfs:label "Vacant or Disused Community Services Site" ;
    skos:narrower <700>,
        <701>,
        <702>,
        <703>,
        <704>,
        <705>,
        <706>,
        <707> ;
    skos:prefLabel "Vacant or Disused Community Services Site" .

<700> a skos:Concept ;
    rdfs:label "Vacant Health Services Development Site" ;
    skos:definition "Vacant land with a permit approved or capable of being developed for health purposes, e.g. hospital site." ;
    skos:prefLabel "Vacant Health Services Development Site" .

<701> a skos:Concept ;
    rdfs:label "Vacant Education and Research Development Site" ;
    skos:definition "Vacant land with a permit approved or capable of being developed for education purposes, e.g. school/university site." ;
    skos:prefLabel "Vacant Education and Research Development Site" .

<702> a skos:Concept ;
    rdfs:label "Vacant Justice and Community Protection Development Site" ;
    skos:definition "Vacant land with a permit approved or capable of being developed for justice and community protection purposes, e.g. police station, court house." ;
    skos:prefLabel "Vacant Justice and Community Protection Development Site" .

<703> a skos:Concept ;
    rdfs:label "Vacant Religious Purposes Development Site" ;
    skos:definition "Vacant land with a permit approved or capable of being developed for religious purposes, e.g. church, temple, synagogue site." ;
    skos:prefLabel "Vacant Religious Purposes Development Site" .

<704> a skos:Concept ;
    rdfs:label "Vacant Community Services Development Site" ;
    skos:definition "Vacant land with a permit approved or capable of being developed for community services, e.g. clubrooms." ;
    skos:prefLabel "Vacant Community Services Development Site" .

<705> a skos:Concept ;
    rdfs:label "Vacant Government Administration Development Site" ;
    skos:definition "Vacant land with a permit approved or capable of being developed for government administration purposes, e.g. civic purposes." ;
    skos:prefLabel "Vacant Government Administration Development Site" .

<706> a skos:Concept ;
    rdfs:label "Vacant Defence Services Development Site" ;
    skos:definition "Vacant land with a permit approved or capable of being developed for defence purposes, e.g. barracks." ;
    skos:prefLabel "Vacant Defence Services Development Site" .

<707> a skos:Concept ;
    rdfs:label "Cemetery" ;
    skos:definition "Land permitted to be used as a cemetery." ;
    skos:prefLabel "Cemetery" .

<71> a skos:Concept ;
    rdfs:label "Health" ;
    skos:narrower <710>,
        <711>,
        <712>,
        <713>,
        <714>,
        <715> ;
    skos:prefLabel "Health" .

<710> a skos:Concept ;
    rdfs:label "Public Hospital" ;
    skos:definition "Land developed and used as a hospital funded by the government for public patients." ;
    skos:prefLabel "Public Hospital" .

<711> a skos:Concept ;
    rdfs:label "Private Hospital" ;
    skos:definition "Land developed and used as a non-government funded hospital for private patients." ;
    skos:prefLabel "Private Hospital" .

<712> a skos:Concept ;
    rdfs:label "Welfare Centre" ;
    skos:definition "Land developed and used for the purposes of providing welfare services to the community." ;
    skos:note "Changed from Infant Welfare Centre to Welfare Centre" ;
    skos:prefLabel "Welfare Centre" .

<713> a skos:Concept ;
    rdfs:label "Community Health Centre" ;
    skos:definition "Land developed and used as consulting facilities, for a range of public health issues to the wider community." ;
    skos:prefLabel "Community Health Centre" .

<714> a skos:Concept ;
    rdfs:label "Centre for the Mentally ill" ;
    skos:definition "Land developed with specialist facilities and used for the treatment of the mentally ill. Includes rehabilitation clinics." ;
    skos:prefLabel "Centre for the Mentally ill" .

<715> a skos:Concept ;
    rdfs:label "Day Care Centre for Children" ;
    skos:definition "Land developed and permitted to be used as a day care centre of children by a licensed operator." ;
    skos:prefLabel "Day Care Centre for Children" .

<72> a skos:Concept ;
    rdfs:label "Education and Research" ;
    skos:narrower <720>,
        <721>,
        <722>,
        <723>,
        <724>,
        <725>,
        <726>,
        <727>,
        <728>,
        <729> ;
    skos:prefLabel "Education and Research" .

<720> a skos:Concept ;
    rdfs:label "Early Childhood Development Centre – Kindergarten" ;
    skos:definition "Land developed and permitted to be used as a funded early education centre for children 3-5 year olds." ;
    skos:narrower <720.1>,
        <720.2>,
        <720.3>,
        <720.4>,
        <720.5> ;
    skos:prefLabel "Early Childhood Development Centre – Kindergarten" .

<720.1> a skos:Concept ;
    rdfs:label "Unspecified" ;
    skos:prefLabel "Unspecified" .

<720.2> a skos:Concept ;
    rdfs:label "Early Childhood Development Centre" ;
    skos:prefLabel "Early Childhood Development Centre" .

<720.3> a skos:Concept ;
    rdfs:label "Kindergarten" ;
    skos:prefLabel "Kindergarten" .

<720.4> a skos:Concept ;
    rdfs:label "Pre-School" ;
    skos:prefLabel "Pre-School" .

<720.5> a skos:Concept ;
    rdfs:label "Child Welfare and Pre-School" ;
    skos:prefLabel "Child Welfare and Pre-School" .

<721> a skos:Concept ;
    rdfs:label "Government School" ;
    skos:definition "Land developed and used in the education of students in a government school operated by the state." ;
    skos:narrower <721.1>,
        <721.2>,
        <721.3>,
        <721.4>,
        <721.5>,
        <721.6> ;
    skos:note "Changed from School Primary – Public/Private to Government School" ;
    skos:prefLabel "Government School" .

<721.1> a skos:Concept ;
    rdfs:label "Unspecified" ;
    skos:note "New AVPCC - subclassification" ;
    skos:prefLabel "Unspecified" .

<721.2> a skos:Concept ;
    rdfs:label "Primary School" ;
    skos:definition "Land developed and used in the education of students in years p-6/7." ;
    skos:note "New AVPCC - subclassification" ;
    skos:prefLabel "Primary School" .

<721.3> a skos:Concept ;
    rdfs:label "Secondary School/College" ;
    skos:definition "Land developed and used in the education of students in years 7/8-12. Includes trade and technical schools." ;
    skos:note "New AVPCC - subclassification" ;
    skos:prefLabel "Secondary School/College" .

<721.4> a skos:Concept ;
    rdfs:label "Combined Primary/Secondary" ;
    skos:definition "Land developed and used in the education of students in years p-12." ;
    skos:note "New AVPCC - subclassification" ;
    skos:prefLabel "Combined Primary/Secondary" .

<721.5> a skos:Concept ;
    rdfs:label "Technical School" ;
    skos:definition "Land developed and used in the education of students in years 7/8-12 for trade and technical purposes." ;
    skos:note "New AVPCC - subclassification" ;
    skos:prefLabel "Technical School" .

<721.6> a skos:Concept ;
    rdfs:label "Playing Fields and Sporting Facilities" ;
    skos:note "New AVPCC - subclassification" ;
    skos:prefLabel "Playing Fields and Sporting Facilities" .

<722> a skos:Concept ;
    rdfs:label "School Camps" ;
    skos:definition "Land developed and used as a camp exclusively for the education of students by a registered education provider." ;
    skos:note "New AVPCC" ;
    skos:prefLabel "School Camps" .

<723> a skos:Concept ;
    rdfs:label "Non-Government School" ;
    skos:definition "Land developed and used in the education of students in a non-government school operated by a registered education provider." ;
    skos:narrower <723.1>,
        <723.2>,
        <723.3>,
        <723.4>,
        <723.5>,
        <723.6> ;
    skos:note "Changed from School/College Secondary/Technical School  Public/Private to Non Government School" ;
    skos:prefLabel "Non-Government School" .

<723.1> a skos:Concept ;
    rdfs:label "Unspecified" ;
    skos:note "New AVPCC - subclassification" ;
    skos:prefLabel "Unspecified" .

<723.2> a skos:Concept ;
    rdfs:label "Primary School" ;
    skos:definition "Land developed and used in the education of students in years p-6/7." ;
    skos:note "New AVPCC - subclassification" ;
    skos:prefLabel "Primary School" .

<723.3> a skos:Concept ;
    rdfs:label "Secondary School/College" ;
    skos:definition "Land developed and used in the education of students in years 7/8-12." ;
    skos:note "New AVPCC - subclassification" ;
    skos:prefLabel "Secondary School/College" .

<723.4> a skos:Concept ;
    rdfs:label "Combined Primary/Secondary" ;
    skos:definition "Land developed and used in the education of students in years p-12." ;
    skos:note "New AVPCC - subclassification" ;
    skos:prefLabel "Combined Primary/Secondary" .

<723.5> a skos:Concept ;
    rdfs:label "Technical School" ;
    skos:definition "Land developed and used in the education of students in years 7/8-12 for trade and technical purposes." ;
    skos:note "New AVPCC - subclassification" ;
    skos:prefLabel "Technical School" .

<723.6> a skos:Concept ;
    rdfs:label "Playing Fields and Sporting Facilities" ;
    skos:note "New AVPCC - subclassification" ;
    skos:prefLabel "Playing Fields and Sporting Facilities" .

<724> a skos:Concept ;
    rdfs:label "Special Needs School" ;
    skos:definition "Land developed and used in the education of pupils with special needs by a registered education provider." ;
    skos:prefLabel "Special Needs School" .

<725> a skos:Concept ;
    rdfs:label "University" ;
    skos:definition "Land developed and used in undergraduate and post graduate studies at degree, masters and PhD levels by a registered university." ;
    skos:note "Changed from University - Public/Private to University" ;
    skos:prefLabel "University" .

<726> a skos:Concept ;
    rdfs:label "Technical and Further Education" ;
    skos:definition "Land developed and used for post-secondary school education and training by a registered education provider. Usually aimed at developing specific job core competencies." ;
    skos:prefLabel "Technical and Further Education" .

<727> a skos:Concept ;
    rdfs:label "Research Institute – Public" ;
    skos:definition "Land developed and used as a research facility by the government." ;
    skos:prefLabel "Research Institute – Public" .

<728> a skos:Concept ;
    rdfs:label "Observatory" ;
    skos:definition "Land developed with purpose-built infrastructure associated with astronomy and of national scientific importance." ;
    skos:prefLabel "Observatory" .

<729> a skos:Concept ;
    rdfs:label "Residential College/Quarters - Defence forces" ;
    skos:definition "Residential accommodation/quarters for the defence forces." ;
    skos:prefLabel "Residential College/Quarters - Defence forces" .

<73> a skos:Concept ;
    rdfs:label "Justice and Community Protection" ;
    skos:narrower <730>,
        <731>,
        <732>,
        <733>,
        <734>,
        <735>,
        <736> ;
    skos:prefLabel "Justice and Community Protection" .

<730> a skos:Concept ;
    rdfs:label "Police Facility" ;
    skos:definition "Land developed and used as a policing facility, at district/regional/state level." ;
    skos:prefLabel "Police Facility" .

<731> a skos:Concept ;
    rdfs:label "Court Facility" ;
    skos:definition "Land developed and used as a judicial facility for either a Court or tribunal." ;
    skos:prefLabel "Court Facility" .

<732> a skos:Concept ;
    rdfs:label "Prison/Detention Centre/Gaol Complex/ Corrective Institution" ;
    skos:definition "Land developed and used for custodial purposes." ;
    skos:prefLabel "Prison/Detention Centre/Gaol Complex/ Corrective Institution" .

<733> a skos:Concept ;
    rdfs:label "Fire Station Facility" ;
    skos:definition "Land developed and used for the storage of vehicles and equipment for the fighting of fires." ;
    skos:prefLabel "Fire Station Facility" .

<734> a skos:Concept ;
    rdfs:label "Ambulance Station Facility" ;
    skos:definition "Land developed and used as an ambulance station." ;
    skos:prefLabel "Ambulance Station Facility" .

<735> a skos:Concept ;
    rdfs:label "Emergency Services Complex" ;
    skos:definition "Land developed and used for state emergency services facilities." ;
    skos:prefLabel "Emergency Services Complex" .

<736> a skos:Concept ;
    rdfs:label "Community Protection and Services Training Facility" ;
    skos:definition "Land developed and used as a specialist facility for the training of fire, police, ambulance, SES and prison personnel." ;
    skos:prefLabel "Community Protection and Services Training Facility" .

<74> a skos:Concept ;
    rdfs:label "Religious" ;
    skos:narrower <740>,
        <741>,
        <742>,
        <743> ;
    skos:prefLabel "Religious" .

<740> a skos:Concept ;
    rdfs:label "Place of Worship" ;
    skos:definition "Land developed and used as a place of worship." ;
    skos:note "Changed from Church, Temple, Synagogue, etc. to Place of Worship" ;
    skos:prefLabel "Place of Worship" .

<741> a skos:Concept ;
    rdfs:label "Religious Hall" ;
    skos:definition "Land developed and used for the social interaction of people by a religious organisation." ;
    skos:prefLabel "Religious Hall" .

<742> a skos:Concept ;
    rdfs:label "Religious Residence" ;
    skos:definition "Land developed and used as a dwelling by an ordained member/members of a religious order, as part of administering their religious duties." ;
    skos:note "Changed from Rectory, Manse, Presbytery to Religious Residence" ;
    skos:prefLabel "Religious Residence" .

<743> a skos:Concept ;
    rdfs:label "Religious Study Centre" ;
    skos:definition "Land developed and used as a religious study centre." ;
    skos:prefLabel "Religious Study Centre" .

<75> a skos:Concept ;
    rdfs:label "Community Service and Sporting Clubrooms and Halls" ;
    skos:narrower <750>,
        <751>,
        <752> ;
    skos:prefLabel "Community Service and Sporting Clubrooms and Halls" .

<750> a skos:Concept ;
    rdfs:label "Halls and Service Clubrooms" ;
    skos:definition "Land developed and used as an occasional meeting place by community based groups or clubs." ;
    skos:prefLabel "Halls and Service Clubrooms" .

<751> a skos:Concept ;
    rdfs:label "Rural and Community Camps" ;
    skos:definition "Land developed with accommodation used by persons or groups for short term recreation/training/education purposes by a community service provider e.g. scout camp." ;
    skos:prefLabel "Rural and Community Camps" .

<752> a skos:Concept ;
    rdfs:label "Community Facility" ;
    skos:definition "Land developed and used as a meeting place by groups involved in community interests, e.g. neighbour centre." ;
    skos:note "Changed from Community/Neighbourhood Facility to Community Facility" ;
    skos:prefLabel "Community Facility" .

<76> a skos:Concept ;
    rdfs:label "Government Administration" ;
    skos:narrower <760>,
        <761>,
        <762>,
        <763> ;
    skos:prefLabel "Government Administration" .

<760> a skos:Concept ;
    rdfs:label "Parliament House" ;
    skos:definition "Land developed and used by government as a house of parliament." ;
    skos:prefLabel "Parliament House" .

<761> a skos:Concept ;
    rdfs:label "Government House" ;
    skos:definition "Land developed and used as a residence by a governor of a state or the Commonwealth." ;
    skos:prefLabel "Government House" .

<762> a skos:Concept ;
    rdfs:label "Local Government" ;
    skos:definition "Land developed and used for the administration of local government." ;
    skos:prefLabel "Local Government" .

<763> a skos:Concept ;
    rdfs:label "Civic Buildings" ;
    skos:definition "Land developed and used by local government for civic purposes." ;
    skos:prefLabel "Civic Buildings" .

<77> a skos:Concept ;
    rdfs:label "Defence Services/Military Base" ;
    skos:narrower <770>,
        <771>,
        <772>,
        <773>,
        <774>,
        <775>,
        <776>,
        <777>,
        <778> ;
    skos:prefLabel "Defence Services/Military Base" .

<770> a skos:Concept ;
    rdfs:label "Army Barracks/Administration Base" ;
    skos:definition "Land developed and used for the administration of the armed forces." ;
    skos:prefLabel "Army Barracks/Administration Base" .

<771> a skos:Concept ;
    rdfs:label "Army Maintenance Depots" ;
    skos:definition "Land developed and used by the army for the storage and maintenance of equipment and infrastructure." ;
    skos:prefLabel "Army Maintenance Depots" .

<772> a skos:Concept ;
    rdfs:label "Army Field Camps and Firing Ranges" ;
    skos:definition "Land developed and used by the army as field camps and for firearms training/practice." ;
    skos:prefLabel "Army Field Camps and Firing Ranges" .

<773> a skos:Concept ;
    rdfs:label "Naval Base/Administration Base" ;
    skos:definition "Land developed and used for the administration of the naval forces." ;
    skos:prefLabel "Naval Base/Administration Base" .

<774> a skos:Concept ;
    rdfs:label "Naval Specialised Facilities – Ground Based" ;
    skos:definition "Land developed with specialised infrastructure for use by the navy, e.g. storage, maintenance and training." ;
    skos:prefLabel "Naval Specialised Facilities – Ground Based" .

<775> a skos:Concept ;
    rdfs:label "Naval Specialised Facilities – Water Based" ;
    skos:definition "Land developed with specialised infrastructure associated with the berthing of navy vessels, e.g. wharves, dry docks." ;
    skos:prefLabel "Naval Specialised Facilities – Water Based" .

<776> a skos:Concept ;
    rdfs:label "Air Force Base/Administration" ;
    skos:definition "Land developed and used for the administration of the Air forces." ;
    skos:prefLabel "Air Force Base/Administration" .

<777> a skos:Concept ;
    rdfs:label "Airstrip and Specialised Facilities" ;
    skos:definition "Land developed with specialised infrastructure associated with an airbase used by the Air Force, e.g. airfields, hangars, storage and maintenance." ;
    skos:prefLabel "Airstrip and Specialised Facilities" .

<778> a skos:Concept ;
    rdfs:label "Munitions Storage Facility" ;
    skos:definition "Land developed and used the defence forces for the storage of explosives, ammunition and bombs." ;
    skos:prefLabel "Munitions Storage Facility" .

<78> a skos:Concept ;
    rdfs:label "Other Community service facilities" ;
    skos:narrower <780>,
        <781>,
        <782>,
        <783> ;
    skos:note "Changed from Community service facilities or other to Other Community service facilities" ;
    skos:prefLabel "Other Community service facilities" .

<780> a skos:Concept ;
    rdfs:label "Public Conveniences" ;
    skos:definition "Land developed and used as a public convenience, e.g. public toilet block." ;
    skos:prefLabel "Public Conveniences" .

<781> a skos:Concept ;
    rdfs:label "Unspecified – Public, Education and Health Improved" ;
    skos:definition "Land developed and used for the provision of education and health to the public by community service groups." ;
    skos:prefLabel "Unspecified – Public, Education and Health Improved" .

<782> a skos:Concept ;
    rdfs:label "Unspecified – Public, Education and Health vacant" ;
    skos:definition "Vacant land with a permit approved or capable of being developed for public education and health services." ;
    skos:prefLabel "Unspecified – Public, Education and Health vacant" .

<783> a skos:Concept ;
    rdfs:label "Animal shelter" ;
    skos:definition "Land developed and used as an animal welfare shelter by a community service group. May include keeping the animals on the premises for treatment or adoption" ;
    skos:note "New AVPCC" ;
    skos:prefLabel "Animal shelter" .

<80> a skos:Concept ;
    rdfs:label "Vacant Land" ;
    skos:narrower <800>,
        <801>,
        <802> ;
    skos:prefLabel "Vacant Land" .

<800> a skos:Concept ;
    rdfs:label "Vacant Site – Sporting Use" ;
    skos:definition "Vacant land with a permit approved or capable of being developed for sporting use." ;
    skos:prefLabel "Vacant Site – Sporting Use" .

<801> a skos:Concept ;
    rdfs:label "Vacant Site – Heritage Application" ;
    skos:definition "Vacant land designated and zoned for heritage purposes, e.g. historic precinct, heritage landscape." ;
    skos:prefLabel "Vacant Site – Heritage Application" .

<802> a skos:Concept ;
    rdfs:label "Vacant Site – Cultural Use" ;
    skos:definition "Vacant land designated and zoned for cultural purposes." ;
    skos:prefLabel "Vacant Site – Cultural Use" .

<81> a skos:Concept ;
    rdfs:label "State/Regional Sports Complex" ;
    skos:narrower <810>,
        <811>,
        <812>,
        <813>,
        <814>,
        <815>,
        <816>,
        <817>,
        <818> ;
    skos:note "Changed from State/Regional Sports Complex (Superior Facility) to State/Regional Sports Complex" ;
    skos:prefLabel "State/Regional Sports Complex" .

<810> a skos:Concept ;
    rdfs:label "Major Sports Complex" ;
    skos:definition "Land developed with specialised infrastructure used as a major sporting facility for commercial purposes, e.g. MCG." ;
    skos:note "Changed from Major Sports Facility (full commercial application) to Major Sports Facility" ;
    skos:prefLabel "Major Sports Complex" .

<811> a skos:Concept ;
    rdfs:label "Major Indoor Sports Complex" ;
    skos:definition "Land developed with specialised infrastructure used as an indoor sporting facility for commercial purposes, e.g. Rod Laver Arena." ;
    skos:note "Changed from Indoor Sports Grounds/Complex (includes stadiums, arenas, velodromes etc. – usually state/regional centre with likely some commercial application) to Major Indoor Sports Facility" ;
    skos:prefLabel "Major Indoor Sports Complex" .

<812> a skos:Concept ;
    rdfs:label "Outdoor\\Indoor Sports Complex - non major" ;
    skos:definition "Land developed and used as a state or regional sports facility with limited commercial application, e.g.  Velodrome, Netball Hockey centre." ;
    skos:note "Changed from Outdoor Sports Grounds/Complex (includes stadiums, arenas, courts etc. – usually state/regional centre with likely some commercial application) to Outdoor Sports Complex" ;
    skos:prefLabel "Outdoor\\Indoor Sports Complex - non major" .

<813> a skos:Concept ;
    rdfs:label "Outdoor Sports – Extended Areas/Cross Country" ;
    skos:definition "Land developed with specialist infrastructure over extended open areas used for recreational/sporting activities, e.g. member facility golf course, polo fields." ;
    skos:note "Changed from Outdoor Sports – Extended Areas/Cross Country (likely some commercial application) to Outdoor Sports – Extended Areas/Cross Country" ;
    skos:prefLabel "Outdoor Sports – Extended Areas/Cross Country" .

<814> a skos:Concept ;
    rdfs:label "Aquatic Complex" ;
    skos:definition "Land developed with specialised infrastructure used as an aquatic complex for water sports." ;
    skos:note "Changed from Water Sports – Confined Areas (likely some commercial application) to Aquatic Complex" ;
    skos:prefLabel "Aquatic Complex" .

<815> a skos:Concept ;
    rdfs:label "Water Sports – Outdoor" ;
    skos:definition "Land developed with specialised infrastructure used for open air water sports, e.g. rowing." ;
    skos:note "Changed from Water Sports – Open Areas (likely some commercial application) to Water Sports – Outdoor" ;
    skos:prefLabel "Water Sports – Outdoor" .

<816> a skos:Concept ;
    rdfs:label "Motor Racing Tracks/Speedways" ;
    skos:definition "Land developed with specialised infrastructure used for motor sports." ;
    skos:note "Changed from Motor Racing Tracks/Speedways (likely some commercial application) to Motor Racing Tracks/Speedways" ;
    skos:prefLabel "Motor Racing Tracks/Speedways" .

<817> a skos:Concept ;
    rdfs:label "Racecourse/Tracks" ;
    skos:definition "Land developed with specialised infrastructure used for horse, greyhound, or harness racing, e.g. Flemington, Randwick." ;
    skos:note "Changed from Racecourse/Tracks/Showground (sport involving animals, likely some commercial application) to Racecourse/Tracks" ;
    skos:prefLabel "Racecourse/Tracks" .

<818> a skos:Concept ;
    rdfs:label "Ski Fields" ;
    skos:definition "Land developed with specialised infrastructure used as a ski area for commercial purposes. Includes a field, run, trail or course prepared for the purpose of alpine recreation." ;
    skos:note "Changed from Ski Fields (likely some commercial application) to Ski Fields" ;
    skos:prefLabel "Ski Fields" .

<82> a skos:Concept ;
    rdfs:label "Local Sporting Facilities" ;
    skos:narrower <820>,
        <821>,
        <822>,
        <823>,
        <824>,
        <825>,
        <826>,
        <827>,
        <828>,
        <829> ;
    skos:prefLabel "Local Sporting Facilities" .

<820> a skos:Concept ;
    rdfs:label "Indoor Sports Centre" ;
    skos:definition "Land developed and used as a local indoor recreational facility." ;
    skos:narrower <820.1>,
        <820.2>,
        <820.3>,
        <820.4>,
        <820.5> ;
    skos:note "Changed from Indoor Sports Centre etc. (includes gymnasiums, stadiums/courts etc.) to Indoor Sports Centre" ;
    skos:prefLabel "Indoor Sports Centre" .

<820.1> a skos:Concept ;
    rdfs:label "Unspecified" ;
    skos:prefLabel "Unspecified" .

<820.2> a skos:Concept ;
    rdfs:label "Squash Courts" ;
    skos:prefLabel "Squash Courts" .

<820.3> a skos:Concept ;
    rdfs:label "Gymnasium/Health Club" ;
    skos:prefLabel "Gymnasium/Health Club" .

<820.4> a skos:Concept ;
    rdfs:label "Indoor Sports Complex" ;
    skos:prefLabel "Indoor Sports Complex" .

<820.5> a skos:Concept ;
    rdfs:label "Bowling Alley" ;
    skos:prefLabel "Bowling Alley" .

<821> a skos:Concept ;
    rdfs:label "Outdoor Sports Grounds town or suburban facilities" ;
    skos:definition "Land developed and used as a local outdoor recreation facility." ;
    skos:narrower <821.1>,
        <821.2>,
        <821.3>,
        <821.4> ;
    skos:prefLabel "Outdoor Sports Grounds town or suburban facilities" .

<821.1> a skos:Concept ;
    rdfs:label "Unspecified" ;
    skos:prefLabel "Unspecified" .

<821.2> a skos:Concept ;
    rdfs:label "Tennis Club" ;
    skos:prefLabel "Tennis Club" .

<821.3> a skos:Concept ;
    rdfs:label "Bowling Club" ;
    skos:prefLabel "Bowling Club" .

<821.4> a skos:Concept ;
    rdfs:label "Outdoor Park and Facilities" ;
    skos:prefLabel "Outdoor Park and Facilities" .

<822> a skos:Concept ;
    rdfs:label "Outdoor Sports – Extended Areas/Cross Country" ;
    skos:definition "Land developed with specialist infrastructure over extended open areas used for local recreational/sporting activities, e.g. municipal golf course." ;
    skos:prefLabel "Outdoor Sports – Extended Areas/Cross Country" .

<823> a skos:Concept ;
    rdfs:label "Swimming Pools/Aquatic Centres" ;
    skos:definition "Land developed with specialised infrastructure used as a local aquatic complex for water sports, e.g. municipal swimming centre." ;
    skos:note "Changed from Water Sports – Swimming Pools/Aquatic Centres to Swimming Pools/Aquatic Centres" ;
    skos:prefLabel "Swimming Pools/Aquatic Centres" .

<824> a skos:Concept ;
    rdfs:label "Water Sports – Outdoor" ;
    skos:definition "Land developed with specialised infrastructure used for local open air water sports, e.g. rowing." ;
    skos:note "Changed from Water Sports – Open Areas to Water Sports – Outdoor" ;
    skos:prefLabel "Water Sports – Outdoor" .

<825> a skos:Concept ;
    rdfs:label "Motor Race Tracks/Speedways" ;
    skos:definition "Land developed with specialised infrastructure used for local motor sports." ;
    skos:prefLabel "Motor Race Tracks/Speedways" .

<826> a skos:Concept ;
    rdfs:label "Aero Club Facility" ;
    skos:definition "Land used by aero clubs for flying pursuits. May include aircraft hangers." ;
    skos:note "New AVPCC" ;
    skos:prefLabel "Aero Club Facility" .

<827> a skos:Concept ;
    rdfs:label "Ski Fields" ;
    skos:definition "Land developed with limited infrastructure and used for recreational alpine pursuits. Limited commercial application." ;
    skos:prefLabel "Ski Fields" .

<828> a skos:Concept ;
    rdfs:label "Equestrian Centre" ;
    skos:definition "Land developed with specialised infrastructure used for the grooming and showing of horses." ;
    skos:prefLabel "Equestrian Centre" .

<829> a skos:Concept ;
    rdfs:label "Bike Track/Walking Trails" ;
    skos:definition "Land designated as a bike track/walking trail." ;
    skos:prefLabel "Bike Track/Walking Trails" .

<83> a skos:Concept ;
    rdfs:label "National/State Cultural Heritage Centres" ;
    skos:narrower <830>,
        <831>,
        <832>,
        <833>,
        <834>,
        <835>,
        <836>,
        <837> ;
    skos:note "Changed from National/State/Regional Cultural Heritage Centres to National/State Cultural Heritage Centres" ;
    skos:prefLabel "National/State Cultural Heritage Centres" .

<830> a skos:Concept ;
    rdfs:label "Library/Archives" ;
    skos:definition "Land developed and used as a library or archival facility with state or national significance." ;
    skos:prefLabel "Library/Archives" .

<831> a skos:Concept ;
    rdfs:label "Museum/Art Gallery" ;
    skos:definition "Land developed and used as a Museum/Art Gallery with state or national significance." ;
    skos:prefLabel "Museum/Art Gallery" .

<832> a skos:Concept ;
    rdfs:label "Cultural Heritage Centre" ;
    skos:definition "Land developed and used as a cultural heritage centre with state or national significance." ;
    skos:prefLabel "Cultural Heritage Centre" .

<833> a skos:Concept ;
    rdfs:label "Wildlife Zoo" ;
    skos:definition "Land developed and used as zoological gardens with state or national significance." ;
    skos:note "Changed from Wildlife Zoo/Aquarium to Wildlife Zoo" ;
    skos:prefLabel "Wildlife Zoo" .

<834> a skos:Concept ;
    rdfs:label "Aquarium" ;
    skos:definition "Land developed and used as an aquarium with state or national significance." ;
    skos:prefLabel "Aquarium" .

<835> a skos:Concept ;
    rdfs:label "Botanical Gardens" ;
    skos:definition "Land developed and used as botanical gardens with state or national significance." ;
    skos:prefLabel "Botanical Gardens" .

<836> a skos:Concept ;
    rdfs:label "Monument/Memorial" ;
    skos:definition "Land developed and used as a monument/memorial with state or national significance, e.g. Shrine of Remembrance." ;
    skos:prefLabel "Monument/Memorial" .

<837> a skos:Concept ;
    rdfs:label "Culture, recreation and sport" ;
    skos:definition "Land developed and used as a culture, recreation and sport centre with state or national significance." ;
    skos:prefLabel "Culture, recreation and sport" .

<84> a skos:Concept ;
    rdfs:label "Local Cultural Heritage Sites, Memorials and Monuments" ;
    skos:narrower <840>,
        <841>,
        <842>,
        <843>,
        <844>,
        <845> ;
    skos:prefLabel "Local Cultural Heritage Sites, Memorials and Monuments" .

<840> a skos:Concept ;
    rdfs:label "Library/Archives" ;
    skos:definition "Land developed and used as a library or archival facility with local significance." ;
    skos:prefLabel "Library/Archives" .

<841> a skos:Concept ;
    rdfs:label "Museum/Art Gallery" ;
    skos:definition "Land developed and used as a Museum/Art Gallery with local significance." ;
    skos:prefLabel "Museum/Art Gallery" .

<842> a skos:Concept ;
    rdfs:label "Cultural Heritage Centre" ;
    skos:definition "Land developed and used as a cultural heritage centre with local significance." ;
    skos:prefLabel "Cultural Heritage Centre" .

<843> a skos:Concept ;
    rdfs:label "Wildlife Zoo/Park/Aquarium" ;
    skos:definition "Land developed and used as a wildlife zoo/aquarium with local significance." ;
    skos:prefLabel "Wildlife Zoo/Park/Aquarium" .

<844> a skos:Concept ;
    rdfs:label "Parks and Gardens" ;
    skos:definition "Land developed and used as parks and gardens with local significance." ;
    skos:prefLabel "Parks and Gardens" .

<845> a skos:Concept ;
    rdfs:label "Monument/Memorial" ;
    skos:definition "Land developed and used as a monument/memorial with local significance." ;
    skos:prefLabel "Monument/Memorial" .

<85> a skos:Concept ;
    rdfs:label "Local Recreation - Other" ;
    skos:narrower <850>,
        <851> ;
    skos:note "New Category" ;
    skos:prefLabel "Local Recreation - Other" .

<850> a skos:Concept ;
    rdfs:label "Bathing Boxes" ;
    skos:definition "Land developed on the foreshore and used as a bathing box for recreational purposes." ;
    skos:note "New AVPCC formally 686 Boat Sheds, Bathing Boxes, Ramps and Jetties" ;
    skos:prefLabel "Bathing Boxes" .

<851> a skos:Concept ;
    rdfs:label "Boat Sheds" ;
    skos:definition "Land developed on the foreshore and used as a boat shed for recreational purposes." ;
    skos:note "New AVPCC formally 686 Boat Sheds, Bathing Boxes, Ramps and Jetties" ;
    skos:prefLabel "Boat Sheds" .

<90> a skos:Concept ;
    rdfs:label "Reserved Land" ;
    skos:narrower <900> ;
    skos:prefLabel "Reserved Land" .

<900> a skos:Concept ;
    rdfs:label "Vacant Land" ;
    skos:definition "Vacant land with special conservation values designated but not proclaimed as a reserve." ;
    skos:note "Changed from Vacant Land (future reserve etc.) to Vacant Land" ;
    skos:prefLabel "Vacant Land" .

<91> a skos:Concept ;
    rdfs:label "Nature Reserve" ;
    skos:narrower <910> ;
    skos:prefLabel "Nature Reserve" .

<910> a skos:Concept ;
    rdfs:label "Nature Reserve" ;
    skos:definition "Land designated and proclaimed as a nature reserve." ;
    skos:prefLabel "Nature Reserve" .

<92> a skos:Concept ;
    rdfs:label "Wilderness Area" ;
    skos:narrower <920>,
        <921> ;
    skos:prefLabel "Wilderness Area" .

<920> a skos:Concept ;
    rdfs:label "World Heritage Area" ;
    skos:definition "Land designated and proclaimed as a world heritage area. Recognised internationally for its unique wilderness values." ;
    skos:prefLabel "World Heritage Area" .

<921> a skos:Concept ;
    rdfs:label "Local Wilderness Area" ;
    skos:definition "Land designated and recognised as a local wilderness area." ;
    skos:prefLabel "Local Wilderness Area" .

<93> a skos:Concept ;
    rdfs:label "National Park (Land and Marine)" ;
    skos:narrower <930>,
        <931> ;
    skos:prefLabel "National Park (Land and Marine)" .

<930> a skos:Concept ;
    rdfs:label "National Park – Land" ;
    skos:definition "Land designated and proclaimed as a national park." ;
    skos:prefLabel "National Park – Land" .

<931> a skos:Concept ;
    rdfs:label "National Park – Marine" ;
    skos:definition "Land designated and proclaimed as a national marine park." ;
    skos:prefLabel "National Park – Marine" .

<94> a skos:Concept ;
    rdfs:label "Natural Monument/Feature" ;
    skos:narrower <940>,
        <941> ;
    skos:prefLabel "Natural Monument/Feature" .

<940> a skos:Concept ;
    rdfs:label "Natural Monument – Land" ;
    skos:definition "Land recognised for its renowned features/scenic/natural/cultural values, e.g. Three Sisters." ;
    skos:prefLabel "Natural Monument – Land" .

<941> a skos:Concept ;
    rdfs:label "Natural Monument – Marine" ;
    skos:definition "Land recognised for its marine features/scenic/cultural values, e.g. Twelve Apostles – Victoria." ;
    skos:prefLabel "Natural Monument – Marine" .

<95> a skos:Concept ;
    rdfs:label "Natural Forests and Forest Reserves" ;
    skos:narrower <950>,
        <951> ;
    skos:prefLabel "Natural Forests and Forest Reserves" .

<950> a skos:Concept ;
    rdfs:label "Forest Reserves – Public" ;
    skos:definition "Public land reserved for the preservation or protection of aesthetic, scientific, flora or fauna values." ;
    skos:prefLabel "Forest Reserves – Public" .

<951> a skos:Concept ;
    rdfs:label "Forest Reserves – Private" ;
    skos:definition "Private land reserved for the preservation or protection of aesthetic, scientific, flora or fauna values." ;
    skos:prefLabel "Forest Reserves – Private" .

<96> a skos:Concept ;
    rdfs:label "Conservation Area" ;
    skos:narrower <960>,
        <961> ;
    skos:prefLabel "Conservation Area" .

<960> a skos:Concept ;
    rdfs:label "Conservation Area – Public" ;
    skos:definition "Public land predominantly in a natural state designated as a conservation area." ;
    skos:prefLabel "Conservation Area – Public" .

<961> a skos:Concept ;
    rdfs:label "Conservation Area – Private" ;
    skos:definition "Private land predominantly in a natural state designated as a conservation area." ;
    skos:prefLabel "Conservation Area – Private" .

<97> a skos:Concept ;
    rdfs:label "Protected Landscape/Seascape" ;
    skos:narrower <970>,
        <971>,
        <972>,
        <973> ;
    skos:prefLabel "Protected Landscape/Seascape" .

<970> a skos:Concept ;
    rdfs:label "Protected Landscape – Public" ;
    skos:definition "Public land designated as a protected landscape recognised for its natural and cultural values." ;
    skos:prefLabel "Protected Landscape – Public" .

<971> a skos:Concept ;
    rdfs:label "Protected Landscape – Private" ;
    skos:definition "Private land designated as a protected landscape recognised for its natural and cultural values." ;
    skos:prefLabel "Protected Landscape – Private" .

<972> a skos:Concept ;
    rdfs:label "Protected Seascape – Public" ;
    skos:definition "Public land designated as a protected seascape recognised for its natural and cultural values." ;
    skos:prefLabel "Protected Seascape – Public" .

<973> a skos:Concept ;
    rdfs:label "Protected Seascape – Private" ;
    skos:definition "Private land designated as a protected seascape recognised for its natural and cultural values." ;
    skos:note "Changed from Protected Landscape – Private to Protected Seascape – Private" ;
    skos:prefLabel "Protected Seascape – Private" .

<98> a skos:Concept ;
    rdfs:label "Wetlands" ;
    skos:narrower <980>,
        <981>,
        <982>,
        <983>,
        <984>,
        <985>,
        <986>,
        <987>,
        <988> ;
    skos:prefLabel "Wetlands" .

<980> a skos:Concept ;
    rdfs:label "River Reserve (fresh water)" ;
    skos:definition "Land designated as a freshwater river reserve, usually with all year round flows." ;
    skos:prefLabel "River Reserve (fresh water)" .

<981> a skos:Concept ;
    rdfs:label "Creek Reserve (fresh water)" ;
    skos:definition "Land designated as a fresh water creek reserve with intermittent flows and tides." ;
    skos:prefLabel "Creek Reserve (fresh water)" .

<982> a skos:Concept ;
    rdfs:label "River Reserve (salt water)" ;
    skos:definition "Land designated as a salt water river reserve, usually with all year round flows." ;
    skos:prefLabel "River Reserve (salt water)" .

<983> a skos:Concept ;
    rdfs:label "Creek Reserve (salt water)" ;
    skos:definition "Land designated as a salt water creek reserve with intermittent flows and tides." ;
    skos:prefLabel "Creek Reserve (salt water)" .

<984> a skos:Concept ;
    rdfs:label "Floodway Reserve" ;
    skos:definition "Land designated as a floodway reserve." ;
    skos:prefLabel "Floodway Reserve" .

<985> a skos:Concept ;
    rdfs:label "Fresh Water Lake Reserve" ;
    skos:definition "Land designated as a fresh water lake reserve that usually holds water all year round." ;
    skos:prefLabel "Fresh Water Lake Reserve" .

<986> a skos:Concept ;
    rdfs:label "Salt Water Lake Reserve" ;
    skos:definition "Land designated as a salt water lake reserve and is not used for commercial salt extraction." ;
    skos:prefLabel "Salt Water Lake Reserve" .

<987> a skos:Concept ;
    rdfs:label "Inland Low Lying Tidal Estuary Wetlands Reserve" ;
    skos:definition "Land designated as a wetlands reserve associated with enclosed bays/salt water river estuary." ;
    skos:prefLabel "Inland Low Lying Tidal Estuary Wetlands Reserve" .

<988> a skos:Concept ;
    rdfs:label "Seabed – Open Sea/Ocean/Bays" ;
    skos:definition "Open sea below high water mark, not being a marine park." ;
    skos:note "Changed from Seabed – Open Sea/Ocean/Bays (not included in the above) to Seabed – Open Sea/Ocean/Bays" ;
    skos:prefLabel "Seabed – Open Sea/Ocean/Bays" .

<99> a skos:Concept ;
    rdfs:label "Game/Fauna Reserves" ;
    skos:narrower <990>,
        <991> ;
    skos:prefLabel "Game/Fauna Reserves" .

<990> a skos:Concept ;
    rdfs:label "Game Reserve – Public" ;
    skos:definition "Public land designated as a game reserve. Hunting of game may be permitted." ;
    skos:prefLabel "Game Reserve – Public" .

<991> a skos:Concept ;
    rdfs:label "Game Reserve – Private" ;
    skos:definition "Private land designated as a game reserve. Hunting of game may be permitted." ;
    skos:prefLabel "Game Reserve – Private" .
